Verified basic SR checker

Experiments/ProofChecking/Array.lean
@@ -1,10 +1,136 @@
 import Std
 import Init.Data.Nat.Basic
 import LeanSAT.Upstream.ToStd
+import Std.Data.List.Init.Lemmas
+
+@[simp] def comm_in_second_arg (f : β → α → β) : Prop :=
+  ∀ (b : β) (a₁ a₂ : α), f (f b a₁) a₂ = f (f b a₂) a₁
+
+namespace List
+
+-- Cayden notes: making a List.foldlIdxM is hard, because the Fin type would be fixed on
+-- the original input L, but would essentially be 0 at each point.
+
+theorem foldl_of_comm (L : List α) (f : β → α → β) (init : β) :
+    comm_in_second_arg f →
+    ∀ a ∈ L, ∃ (acc : β), L.foldl f init = f acc a := by
+  intro hf
+  induction L with
+  | nil => simp
+  | cons x xs ih =>
+    intro a ha
+    rcases List.mem_cons.mp ha with (rfl | ha)
+    · simp
+      sorry
+      done
+    sorry
+    done
+  done
+
+end List
 
 namespace Array
 
 open Nat
+
+theorem Array.ne_empty_iff_size_pos {A : Array α} : A ≠ #[] ↔ 0 < A.size := by
+  have ⟨A⟩ := A
+  have : #[] = ({ data := [] } : Array α) := rfl
+  simp [this]
+  exact Iff.symm List.length_pos
+
+theorem mem_data_iff_exists_fin {A : Array α} {a : α} :
+    a ∈ A.data ↔ ∃ (i : Fin A.size), A[i] = a := by
+  constructor
+  · exact List.get_of_mem
+  · rintro ⟨i, rfl⟩
+    exact Array.getElem_mem_data A i.isLt
+
+@[simp] theorem Array.foldlM_empty {m : Type v → Type w} [Monad m] (f : β → α → m β)
+    (init : β) (start stop : Nat) :
+    Array.foldlM f init #[] start stop = pure init := by
+  simp [foldlM, Id.run]
+  by_cases h : stop = 0
+  · simp [h, foldlM.loop]
+  · simp [h]; simp [foldlM.loop]
+
+@[simp] theorem Array.foldlM_nil {m : Type v → Type w} [Monad m] (f : β → α → m β)
+    (init : β) (start stop : Nat) :
+    Array.foldlM f init { data := [] } start stop = pure init :=
+  Array.foldlM_empty f init start stop
+
+@[simp] theorem Array.foldlM_cons {m : Type v → Type w} [Monad m] (f : β → α → m β)
+    (init : β) (a : α) (as : List α) :
+    Array.foldlM f init { data := a :: as } 0 (size { data := a :: as }) = do
+      { Array.foldlM f (← f init a) { data := as } 0 (size { data := as }) } := by
+  simp only [foldlM_eq_foldlM_data, List.foldlM]
+
+-- TODO: A better implementation exists, probably by writing a custom looper/recursive function
+def foldlIdxM {α : Type u} {β : Type v} {m : Type v → Type w} [Monad m]
+    (as : Array α) (f : β → Fin as.size → α → m β) (init : β) (start := 0) (stop := as.size) : m β :=
+  return Prod.fst <| ← as.foldlM (fun (acc, idx) a =>
+    -- Cayden TODO: Should this be stop instead of as.size?
+    if hidx : idx < as.size then
+      return (← f acc ⟨idx, hidx⟩ a, idx + 1)
+    else
+      return (acc, 0)) (⟨init, start⟩ : β × Nat) start stop
+
+@[inline]
+def foldlIdx {α : Type u} {β : Type v} (as : Array α) (f : β → Fin as.size → α → β)
+    (init : β) (start := 0) (stop := as.size) : β :=
+  Id.run <| as.foldlIdxM f init start stop
+
+def foldrIdxM {α : Type u} {β : Type v} {m : Type v → Type w} [Monad m]
+    (as : Array α) (f : Fin as.size → α → β → m β) (init : β) (start := as.size) (stop := 0) : m β :=
+  return Prod.fst <| ← (as.foldrM (fun a (acc, idx) =>
+    if hidx : idx - 1 < as.size ∧ idx > stop then
+      return (← f ⟨idx - 1, hidx.1⟩ a acc, idx - 1)
+    else
+      return (acc, 0)) (⟨init, start⟩ : β × Nat) start stop)
+
+@[inline]
+def foldrIdx {α : Type u} {β : Type v} (as : Array α) (f : Fin as.size → α → β → β)
+    (init : β) (start := as.size) (stop := 0) : β :=
+  Id.run <| as.foldrIdxM f init start stop
+
+@[simp]
+theorem foldlIdxM_empty {m : Type v → Type w} [Monad m] [LawfulMonad m]
+    (f : β → Fin 0 → α → m β) (init : β) (start stop : Nat) :
+    Array.foldlIdxM #[] f init start stop = pure init := by
+  simp [foldlIdxM]
+  stop
+  done
+
+@[simp]
+theorem foldlIdxM_nil {m : Type v → Type w} [Monad m] [LawfulMonad m]
+    (f : β → Fin 0 → α → m β) (init : β) (start stop : Nat) :
+    Array.foldlIdxM { data := [] } f init start stop = pure init :=
+  Array.foldlIdxM_empty f init start stop
+
+/-
+@[simp]
+theorem foldlIdxM_cons {m : Type v → Type w} [Monad m] [LawfulMonad m]
+     (a : α) (as : List α) (f : β → Fin (a :: as).length → α → m β) (init : β) :
+    Array.foldlIdxM { data := a :: as } f init 0 (size { data := a :: as }) = do
+      { Array.foldlIdxM { data := as } f (← f init 0 a) 0 (size { data := as }) } := by
+  simp [foldlIdxM] -/
+
+--theorem Array.foldlIdx_index_eq (as : Array α) (f : β → Fin as.size → α → β) (init : β) :
+  --as.foldlIdx = something about Array.enum
+
+theorem foldlIdx_of_comm (A : Array α) (f : β → Fin A.size → α → β) (init : β) :
+    -- Commutativity assumption
+    (∀ (acc : β) (idx₁ idx₂ : Fin A.size),
+      f (f acc idx₁ (A.get idx₁)) idx₂ (A.get idx₂) = f (f acc idx₂ (A.get idx₂)) idx₁ (A.get idx₁)) →
+
+    -- For all indexes, we can move its function application to the end
+    ∀ (idx : Fin A.size), ∃ (acc : β), A.foldlIdx f init = f acc idx (A.get idx) := by sorry
+
+-- TODO: Check to see if a similar theorem exists for lists.
+theorem foldl_of_comm (A : Array α) {f : β → α → β} (init : β) :
+    (∀ (acc : β) (a₁ a₂ : α), f (f acc a₁) a₂ = f (f acc a₂) a₁) →
+    ∀ a ∈ A, ∃ (acc : β), A.foldl f init = f acc a := by sorry
+
 
 /-! # setF - a dynamic sizing setting function for arrays -/
 
