Experiments/ProofChecking/PPA.lean
@@ -46,7 +46,7 @@ where
       have : i.val = n := Nat.eq_of_le_of_lt_succ (not_lt.mp h) i.is_lt
       simp_rw [← this]
       assumption
-  termination_by loop x i h => n - i
+  termination_by n - i
 
 lemma Fin.foldl_induction' (n) (f : α → Fin n → α) (init : α) (P : α → Prop)
     (hInit : P init)
@@ -132,6 +132,7 @@ def litValue? (τ : PPA) (l : ILit) : Option Bool :=
     τ.litValue? (-l) = (τ.litValue? l).map Bool.not := by
   aesop (add norm unfold litValue?)
 
+-- TODO: Make iff?
 theorem litValue?_eq_varValue?_none {τ : PPA} {l : ILit} :
     τ.litValue? l = none → τ.varValue? (toVar l) = none := by
   aesop (add norm unfold litValue?)
@@ -143,6 +144,14 @@ theorem litValue?_eq_varValue?_some {τ : PPA} {l : ILit} {b : Bool} :
 @[simp] theorem litValue?_negate_none_iff {τ : PPA} {l : ILit} :
     τ.litValue? (-l) = none ↔ τ.litValue? l = none := by
   simp [litValue?_negate]
+
+@[simp] theorem litValue?_negate_some_iff {τ : PPA} {l : ILit} {b : Bool} :
+    τ.litValue? (-l) = some b ↔ τ.litValue? l = some (!b) := by
+  cases b <;> simp [litValue?_negate]
+
+@[simp] theorem litValue?_negate_some_iff' {τ : PPA} {l : ILit} {b : Bool} :
+    τ.litValue? (-l) = some !b ↔ τ.litValue? l = some b := by
+  cases b <;> simp [litValue?_negate]
 
 theorem lt_size_of_varValue?_some {τ : PPA} {v : IVar} {b : Bool} :
     τ.varValue? v = some b → v.index < τ.size := by
@@ -441,6 +450,15 @@ theorem lt_reset_generation (τ : PPA) : ∀ i ∈ τ.reset.assignment.data, i.n
   have := τ.le_maxGen i h
   linarith
 
+theorem lt_new_generation (maxVar : Nat) : ∀ i ∈ (new maxVar).assignment.data, i.natAbs < (new maxVar).generation := by
+  intro i h
+  simp [new] at h ⊢
+  induction' maxVar with maxVar ih
+  <;> simp at h
+  rcases h with (rfl | h)
+  · rfl
+  · exact ih h
+
 @[simp]
 theorem varValue?_reset (τ : PPA) (v : IVar) : τ.reset.varValue? v = none := by
   unfold varValue?
@@ -465,6 +483,30 @@ theorem litValue?_reset (τ : PPA) (l : ILit) : (τ.reset).litValue? l = none :=
 theorem toPropFun_reset (τ : PPA) : τ.reset.toPropFun = ⊤ := by
   ext; simp [satisfies_iff_vars]
 
+@[simp]
+theorem varValue?_new (maxVar : Nat) (v : IVar) : (new maxVar).varValue? v = none := by
+  unfold varValue?
+  split
+  . rfl
+  . split
+    . next n hn h =>
+      have : n ∈ (new maxVar).assignment.data := by
+        simp_rw [Array.get?_eq_getElem?, Array.getElem?_eq_data_get?, List.get?_eq_some] at hn
+        have ⟨_, hn⟩ := hn
+        rw [← hn]
+        apply List.get_mem
+      have := lt_new_generation maxVar n this
+      linarith
+    . rfl
+
+@[simp]
+theorem litValue?_new (maxVar : Nat) (l : ILit) : (new maxVar).litValue? l = none := by
+  simp [litValue?, varValue?_new]
+
+@[simp]
+theorem toPropFun_new (maxVar : Nat) : (new maxVar).toPropFun = ⊤ := by
+  ext; simp [satisfies_iff_vars]
+
 /-! ### Lemmas about the `setVar`, `setLit` family -/
 
 section setVar
@@ -478,9 +520,8 @@ theorem varValue?_setVar : (τ.setVar v b).varValue? v = some b := by
 
 theorem varValue?_setVar_of_ne {v v' : IVar} :
     v ≠ v' → ∀ (τ : PPA) (b : Bool), (τ.setVar v b).varValue? v' = τ.varValue? v' := by
-  unfold varValue? setVar
   intro hne
-  simp [Array.getElem?_setF' _ _ _ (mt PNat.natPred_inj.mp hne)]
+  simp [varValue?, setVar,Array.getElem?_setF' _ _ _ (mt PNat.natPred_inj.mp hne)]
 
 @[simp]
 theorem varValue?_setLit : (τ.setLit l).varValue? (toVar l) = some (polarity l) := by
@@ -488,6 +529,14 @@ theorem varValue?_setLit : (τ.setLit l).varValue? (toVar l) = some (polarity l)
 
 @[simp]
 theorem litValue?_setLit : (τ.setLit l).litValue? l = some true := by
+  simp [litValue?, setLit, varValue?_setVar]
+
+@[simp]
+theorem litValue?_setLit_negate : (τ.setLit l).litValue? (-l) = some false := by
+  simp [litValue?, setLit, varValue?_setVar]
+
+@[simp]
+theorem litValue?_setLit_negate' : (τ.setLit (-l)).litValue? l = some false := by
   simp [litValue?, setLit, varValue?_setVar]
 
 @[simp]
@@ -519,9 +568,8 @@ theorem varValue?_setVarFor : (τ.setVarFor v b bumps).varValue? v = some b := b
 theorem varValue?_setVarFor_of_ne {v v' : IVar} :
     v ≠ v' → ∀ (τ : PPA) (b : Bool) (bumps : Nat),
       (τ.setVarFor v b bumps).varValue? v' = τ.varValue? v' := by
-  unfold varValue? setVarFor
   intro hne
-  simp [Array.getElem?_setF' _ _ _ (mt PNat.natPred_inj.mp hne)]
+  simp [varValue?, setVarFor, Array.getElem?_setF' _ _ _ (mt PNat.natPred_inj.mp hne)]
 
 @[simp]
 theorem varValue?_setLitFor : (τ.setLitFor l bumps).varValue? (toVar l) = some (polarity l) := by
@@ -529,6 +577,14 @@ theorem varValue?_setLitFor : (τ.setLitFor l bumps).varValue? (toVar l) = some 
 
 @[simp]
 theorem litValue?_setLitFor : (τ.setLitFor l bumps).litValue? l = some true := by
+  simp [litValue?, setLitFor]
+
+@[simp]
+theorem litValue?_setLitFor_negate : (τ.setLitFor l bumps).litValue? (-l) = some false := by
+  simp [litValue?, setLitFor]
+
+@[simp]
+theorem litValue?_setLitFor_negate' : (τ.setLitFor (-l) bumps).litValue? l = some false := by
   simp [litValue?, setLitFor]
 
 theorem varValue?_setLitFor_of_ne {l : ILit} {v : IVar} : toVar l ≠ v →
@@ -636,7 +692,7 @@ theorem toPropFun_setLit_of_true {τ : PPA} {l : ILit} :
   exact toPropFun_setVar_of_some
 
 -- No matter the status of τ.toPropFun, setting the lit adds it to the PPA.
-theorem toPropFun_setLit_lt (τ : PPA) (l : ILit) :
+theorem toPropFun_setLit_le (τ : PPA) (l : ILit) :
     (τ.setLit l).toPropFun ≤ l := by
   apply entails_ext.mpr
   intro σ hσ
@@ -700,20 +756,43 @@ theorem isSetFor_pos_iff : isSetFor τ v > 0 ↔ isSet τ v := by
 theorem isSet_iff : isSet τ v ↔ τ.varValue? v ≠ none :=
   ⟨id, id⟩
 
+@[simp]
+theorem not_isSet_new (maxVar : Nat) (v : IVar) : ¬isSet (new maxVar) v := by
+  simp [isSet, varValue?_new]
+
 theorem isSetFor_zero_iff {τ : PPA} {v : IVar} :
     isSetFor τ v = 0 ↔ τ.varValue? v = none := by
   cases hv : τ.assignment[v.index]?
   <;> simp [isSetFor, varValue?, hv]
-  · exact τ.generation.property
-  · exact succ_le
+  · exact Nat.sub_eq_zero_of_le τ.generation.property
+  · simp [Nat.sub_eq_zero_iff_le]; rfl
 
 @[simp]
 theorem setVar_isSetFor (τ : PPA) (v : IVar) (b : Bool) : isSetFor (τ.setVar v b) v = 1 := by
   simp [isSetFor, setVar]; cases b <;> simp
 
+theorem setVar_isSetFor_of_ne {v v' : IVar} :
+    v ≠ v' → ∀ τ, isSetFor (τ.setVar v true) v' = isSetFor τ v' := by
+  intro hne
+  simp [isSetFor, setVar, Array.getElem?_setF' _ _ _ (mt PNat.natPred_inj.mp hne)]
+
 @[simp]
 theorem setLit_isSetFor (τ : PPA) (l : ILit) : isSetFor (τ.setLit l) (toVar l) = 1 :=
   setVar_isSetFor _ _ _
+
+@[simp]
+theorem setLit_isSetFor_negate (τ : PPA) (l : ILit) : isSetFor (τ.setLit (-l)) (toVar l) = 1 := by
+  simp [setLit]
+
+theorem setLit_isSetFor_of_ne {l₁ l₂ : ILit} :
+    toVar l₁ ≠ toVar l₂ → isSetFor (τ.setLit l₁) (toVar l₂) = isSetFor τ (toVar l₂) := by
+  intro hne
+  simp [isSetFor, setLit, setVar, Array.getElem?_setF' _ _ _ (mt PNat.natPred_inj.mp hne)]
+
+theorem setLit_isSetFor_of_ne' {l : ILit} {v : IVar} :
+    toVar l ≠ v → isSetFor (τ.setLit l) v = isSetFor τ v := by
+  intro hne
+  simp [isSetFor, setLit, setVar, Array.getElem?_setF' _ _ _ (mt PNat.natPred_inj.mp hne)]
 
 @[simp]
 theorem setVarFor_isSetFor (τ : PPA) (v : IVar) (b : Bool) (bumps : Nat) :
@@ -731,6 +810,73 @@ theorem setLitFor_isSetFor (τ : PPA) (l : ILit) (bumps : Nat) :
   setVarFor_isSetFor _ _ _ _
 
 @[simp]
+theorem setLitFor_isSetFor_negate (τ : PPA) (l : ILit) (bumps : Nat) :
+    isSetFor (τ.setLitFor (-l) bumps) (toVar l) = (bumps + 1) := by
+  simp [setLitFor]
+
+theorem setLitFor_isSetFor_of_ne {l₁ l₂ : ILit} :
+    toVar l₁ ≠ toVar l₂ → ∀ (bumps : Nat),
+      isSetFor (τ.setLitFor l₁ bumps) (toVar l₂) = isSetFor τ (toVar l₂) := by
+  intro hne bumps
+  simp [isSetFor, setLitFor, setVarFor, Array.getElem?_setF' _ _ _ (mt PNat.natPred_inj.mp hne)]
+
+-- TODO: Standardize names
+theorem setLitFor_isSetFor_of_ne' {l : ILit} {v : IVar} :
+    toVar l ≠ v → ∀ (bumps : Nat),
+      isSetFor (τ.setLitFor l bumps) v = isSetFor τ v := by
+  intro hne bumps
+  simp [isSetFor, setLitFor, setVarFor, Array.getElem?_setF' _ _ _ (mt PNat.natPred_inj.mp hne)]
+
+@[simp]
+theorem isSet_setVar (τ : PPA) (v : IVar) (b : Bool) :
+    isSet (τ.setVar v b) v := by
+  cases b <;> simp [isSet, setVar, varValue?]
+
+@[simp]
+theorem isSet_setLit (τ : PPA) (l : ILit) :
+    isSet (τ.setLit l) (toVar l) := by
+  cases hpol : polarity l <;> simp [isSet, setLit, setVar, varValue?, hpol]
+
+theorem isSet_setLit_of_ne {l₁ l₂ : ILit} :
+    toVar l₁ ≠ toVar l₂ → ∀ τ, isSet (τ.setLit l₁) (toVar l₂) = isSet τ (toVar l₂) := by
+  intro hne τ
+  simp [isSet, setLit, setVar, varValue?, Array.getElem?_setF' _ _ _ (mt PNat.natPred_inj.mp hne)]
+
+theorem isSet_setLit_of_ne' {l : ILit} {v : IVar} :
+    toVar l ≠ v → ∀ τ, isSet (τ.setLit l) v = isSet τ v := by
+  intro hne τ
+  simp [isSet, setLit, setVar, varValue?, Array.getElem?_setF' _ _ _ (mt PNat.natPred_inj.mp hne)]
+
+@[simp]
+theorem isSet_setVarFor (τ : PPA) (v : IVar) (b : Bool) (offset : Nat) :
+    isSet (τ.setVarFor v b offset) v := by
+  simp [← isSetFor_pos_iff]
+
+@[simp]
+theorem isSet_setLitFor (τ : PPA) (l : ILit) (offset : Nat) :
+    isSet (τ.setLitFor l offset) (toVar l) := by
+  simp [← isSetFor_pos_iff]
+
+theorem isSet_setLitFor_of_ne {l₁ l₂ : ILit} :
+    toVar l₁ ≠ toVar l₂ → ∀ τ bumps,
+      isSet (τ.setLitFor l₁ bumps) (toVar l₂) = isSet τ (toVar l₂) := by
+  intro hne τ bumps
+  simp_rw [← isSetFor_pos_iff, setLitFor_isSetFor_of_ne hne]
+
+theorem isSet_setLitFor_of_ne' {l : ILit} {v : IVar} :
+    toVar l ≠ v → ∀ τ bumps, isSet (τ.setLitFor l bumps) v = isSet τ v := by
+  intro hne τ bumps
+  simp_rw [← isSetFor_pos_iff, setLitFor_isSetFor_of_ne' hne]
+
+@[simp]
+theorem isSet_reset (τ : PPA) : ∀ (v : IVar), ¬isSet τ.reset v := by
+  simp [isSet, varValue?_reset]
+
+@[simp]
+theorem isSet_new (maxVar : Nat) : ∀ (v : IVar), ¬isSet (new maxVar) v := by
+  simp [isSet, varValue?_new]
+
+@[simp]
 theorem isSetFor_bump {τ : PPA} {v : IVar} :
     isSetFor τ.bump v = isSetFor τ v - 1 := by
   simp [isSetFor, bump, ← sub_add_eq, ← Nat.add_sub_add_right]
@@ -739,7 +885,104 @@ theorem isSetFor_bump {τ : PPA} {v : IVar} :
 theorem isSetFor_reset (τ : PPA) (v : IVar) : isSetFor τ.reset v = 0 :=
   isSetFor_zero_iff.mpr (varValue?_reset τ v)
 
+-- CC: This is an iff, but only need → for now
+theorem varValue?_bump_of_isSetFor_pos {τ : PPA} {v : IVar} :
+    isSetFor τ v > 1 → (τ.bump).varValue? v = τ.varValue? v := by
+  intro h
+  simp [varValue?, bump, isSetFor] at h ⊢
+  match hv : τ.assignment[v.index]? with
+  | none => rfl
+  | some g =>
+    simp [hv] at h
+    simp
+    have : (τ.generation.val) + 1 < g.natAbs + 1 := add_lt_of_lt_sub' h
+    have : τ.generation.val + 1 ≤ g.natAbs := lt_succ.mp this
+    have : τ.generation.val ≤ g.natAbs := Nat.le_of_lt this
+    simp [*]
+
 end isSetFor /- section -/
+
+/-! extended and uniform -/
+
+def extended (τ τ' : PPA) (offset : Nat) : Prop := ∀ (v : IVar),
+    (τ.isSet v → τ'.isSetFor v = τ.isSetFor v ∧ τ'.varValue? v = τ.varValue? v)
+    ∧ (¬τ.isSet v → τ'.isSet v → τ'.isSetFor v = offset + 1)
+
+def uniform (τ : PPA) (offset : Nat) : Prop :=
+  ∀ (v : IVar), τ.isSet v → τ.isSetFor v = offset + 1
+
+@[simp]
+theorem extended_refl (τ : PPA) (offset : Nat) : extended τ τ offset := by
+  simp [extended]; intro v hcon h; exact absurd h hcon
+
+theorem extended_trans {τ₁ τ₂ τ₃ : PPA} {offset : Nat} :
+    extended τ₁ τ₂ offset → extended τ₂ τ₃ offset → extended τ₁ τ₃ offset := by
+  intro h₁ h₂ v
+  constructor
+  · intro hv
+    rcases (h₁ v).1 hv with ⟨h_isSet, h_varValue⟩
+    rw [← h_isSet, ← h_varValue]
+    rw [← isSetFor_pos_iff, ← h_isSet, isSetFor_pos_iff] at hv
+    exact (h₂ v).1 hv
+  · intro hv₁ hv₃
+    by_cases hv₂ : τ₂.isSet v
+    · rw [((h₂ v).1 hv₂).1]
+      exact ((h₁ v).2 hv₁) hv₂
+    · exact (h₂ v).2 hv₂ hv₃
+
+theorem entails_of_extended {τ₁ τ₂ : PPA} {offset : Nat} :
+    extended τ₁ τ₂ offset → τ₂.toPropFun ≤ τ₁ := by
+  intro hext
+  apply entails_ext.mpr
+  intro τ hτ₂
+  rw [satisfies_iff_vars] at hτ₂ ⊢
+  intro v b hv
+  have := (hext v).1
+  simp [isSet_iff, hv] at this
+  exact hτ₂ this.2
+
+theorem extended_setLitFor_of_none {τ : PPA} {l : ILit} :
+    τ.litValue? l = none → ∀ offset, extended τ (τ.setLitFor l offset) offset := by
+  intro hl offset v
+  constructor
+  · intro hv
+    by_cases hvar : (toVar l) = v
+    · rw [isSet_iff] at hv
+      have := litValue?_eq_varValue?_none hl
+      rw [hvar] at this
+      rw [this] at hv
+      contradiction
+    · simp [isSet_setLitFor_of_ne' hvar, hv, setLitFor_isSetFor_of_ne' hvar,
+        varValue?_setLitFor_of_ne hvar]
+  · intro hv hlv
+    by_cases hvar : (toVar l) = v
+    · simp [setLitFor, hvar]
+    · simp [isSet_setLitFor_of_ne' hvar] at hlv
+      exact absurd hlv hv
+
+@[simp]
+theorem uniform_new (maxVar : Nat) (offset : Nat) : uniform (new maxVar) offset := by
+  simp [uniform, isSet, isSetFor, varValue?_new]
+
+@[simp]
+theorem uniform_reset (τ : PPA) (offset : Nat) : uniform τ.reset offset := by
+  simp [uniform, isSet, isSetFor, varValue?_reset]
+
+theorem uniform_of_extended_reset {τ₁ τ₂ : PPA} {offset : Nat} :
+    extended (τ₁.reset) τ₂ offset → uniform τ₂ offset := by
+  simp [extended, uniform]
+
+theorem uniform_of_uniform_of_extended {τ₁ τ₂ : PPA} {offset : Nat} :
+    uniform τ₁ offset → extended τ₁ τ₂ offset → uniform τ₂ offset := by
+  simp [uniform, extended]
+  intro hτ₁ h_ext v hv
+  by_cases isSet τ₁ v <;> aesop
+
+theorem uniform_bump_of_uniform_of_extended {τ₁ τ₂ : PPA} {offset : Nat} :
+    offset > 1 → uniform τ₁ offset → extended τ₁ τ₂ 0 →
+      uniform τ₂.bump (offset - 1) ∧ τ₂.bump.toPropFun = τ₁.toPropFun := by
+  sorry
+  done
 
 /-! Assuming negated clauses -/
 
@@ -788,19 +1031,27 @@ theorem setNegatedClause_cons (τ : PPA) (l : ILit) (ls : List ILit) :
 
 /-! Assuming negation of clause, in an Exceptional way. -/
 
-def assumeNegatedClause (τ : PPA) (C : IClause) : Except Unit PPA :=
+def assumeNegatedClause (τ : PPA) (C : IClause) : Except PPA PPA :=
   C.foldlM (init := τ) (fun τ l =>
     match τ.litValue? l with
     | none       => .ok <| τ.setLit (-l)
     | some false => .ok <| τ
-    | some true  => .error ())
+    | some true  => .error τ)
 
-def assumeNegatedClauseFor (τ : PPA) (C : IClause) (bumps : Nat) : Except Unit PPA :=
+-- Assumes the negation of the clause, where unset literals are set to false
+-- (i.e., their negations are set to true) with the provided offset. If the
+-- provided PPA satisfies the clause, then an error is thrown.
+-- Any literal that is initially set to true, it's "bump" value is untouched.
+def assumeNegatedClauseFor (τ : PPA) (C : IClause) (bumps : Nat) : Except PPA PPA :=
   C.foldlM (init := τ) (fun τ l =>
     match τ.litValue? l with
     | none       => .ok <| τ.setLitFor (-l) bumps
     | some false => .ok <| τ
-    | some true  => .error ())
+    | some true  => .error τ)
+
+section assumeNegatedClause
+
+variable {τ τ' : PPA} {C : IClause} {bumps : Nat}
 
 theorem assumeNegatedClause_eq_assumeNegatedClauseFor (τ : PPA) (C : IClause) :
     τ.assumeNegatedClause C = τ.assumeNegatedClauseFor C 0 := by
@@ -820,20 +1071,21 @@ theorem assumeNegatedClauseFor_nil (τ : PPA) (bumps : Nat) :
     τ.assumeNegatedClauseFor { data := [] } bumps = .ok τ := by
   simp [assumeNegatedClauseFor]; rfl
 
-theorem toPropFun_assumeNegatedClauseFor {τ τ' : PPA} {C : IClause} {bumps : Nat} :
-    (τ.assumeNegatedClauseFor C bumps) = .ok τ' → τ'.toPropFun = ↑τ ⊓ (↑C)ᶜ := by
+theorem assumeNegatedClauseFor_ok :
+    (τ.assumeNegatedClauseFor C bumps) = .ok τ' →
+      τ'.toPropFun = ↑τ ⊓ (↑C)ᶜ ∧ extended τ τ' bumps := by
   have ⟨C⟩ := C
   induction' C with l ls ih generalizing τ
-  · simp; rintro rfl; rfl
-  · simp [assumeNegatedClauseFor, -Array.size_mk]
+  · simp; rintro rfl; simp
+  · simp [assumeNegatedClauseFor, -Array.size_mk] at ih ⊢
     cases hτ : τ.litValue? l
     <;> simp [hτ]
     <;> rw [← inf_assoc]
     · intro h
       rw [← litValue?_negate_none_iff] at hτ
-      have := @ih (τ.setLitFor (-l) bumps) h
-      simp [toPropFun_setLit_of_none hτ] at this
-      rw [this]
+      rcases @ih (τ.setLitFor (-l) bumps) h with ⟨h₁, h₂⟩
+      simp [toPropFun_setLit_of_none hτ] at h₁
+      exact ⟨h₁, extended_trans (extended_setLitFor_of_none hτ _) h₂⟩
     · rename Bool => b
       cases b <;> intro h
       · have := @ih τ h
@@ -841,24 +1093,173 @@ theorem toPropFun_assumeNegatedClauseFor {τ τ' : PPA} {C : IClause} {bumps : N
         rwa [hτ] at this
       · contradiction
 
-theorem assumeNegatedClauseFor_spec {τ τ' : PPA} {C : IClause} {bumps : Nat} :
-    (τ.assumeNegatedClauseFor C bumps) = .ok τ' →
-      ∀ {l : ILit}, (l.toPropFun) ≤ C → τ.litValue? l = none →
-        τ'.isSetFor (toVar l) = bumps + 1 := by sorry
-  /-
+theorem assumeNegatedClauseFor_error :
+    (τ.assumeNegatedClauseFor C bumps) = .error τ' → τ.toPropFun ≤ C := by
   have ⟨C⟩ := C
   induction' C with l ls ih generalizing τ
-  · simp; rintro rfl; intro l hl; exact absurd hl (LitVar.toPropFun_ne_bot l)
+  · simp [toPropFun_ne_bot]
   · simp [assumeNegatedClauseFor, -Array.size_mk]
     cases hτ : τ.litValue? l
     <;> simp [hτ]
-    · intro h l' hl'
-      have := ih h
+    <;> intro h
+    · have := ih h
+      rw [← litValue?_negate_none_iff] at hτ
+      simp [toPropFun_setLit_of_none hτ] at this
+      exact sdiff_le_iff.mp this
+    · rename Bool => b
+      cases b
+      · exact le_sup_of_le_right (ih h)
+      · rw [litValue?_true_iff] at hτ
+        exact le_sup_of_le_left hτ
 
-      --rw [satisfies_conj] at hl'
-      done
-    done
-  done -/
+-- TODO: Is this used?
+theorem assumeNegatedClauseFor_error_of_le {τ : PPA} {C : IClause} (bumps : Nat) :
+    τ.toPropFun ≤ C → ∃ τ', (τ.assumeNegatedClauseFor C bumps) = .error τ' := by
+  have ⟨C⟩ := C
+  induction' C with l ls ih generalizing τ
+  · simp [toPropFun_ne_bot]
+  · simp [assumeNegatedClauseFor, -Array.size_mk]
+    intro h
+    cases hτ : τ.litValue? l
+    · have : toPropFun (setLitFor τ (-l) bumps) = τ.toPropFun ⊓ lᶜ := by
+        rw [← litValue?_negate_none_iff] at hτ
+        simp [toPropFun_setLit_of_none hτ]
+      replace h := inf_compl_le_iff_le_sup.mpr h
+      rw [← this] at h
+      exact ih h
+    · rename Bool => b
+      cases b
+      · rw [← inf_compl_le_iff_le_sup, ← litValue?_false_iff_eq_inf.mp hτ] at h
+        exact ih h
+      · simp [hτ]; exact ⟨τ, rfl⟩
+
+-- CC: Ideally we'd say l ≤ C as a stand-in for ∈, but if C is a tautology,
+--     then this applies for all literals. Of course, if C is a tautology,
+--     then assumeNegatedClause returns error instead of ok, but setting
+--     that up for this theorem seems like overkill.
+-- CC TODO: Lots of duplication. Clean up with lemmas later.
+-- TODO: Remove?
+theorem assumeNegatedClauseFor_ok_spec {τ τ' : PPA} {C : IClause} {bumps : Nat} :
+    (τ.assumeNegatedClauseFor C bumps) = .ok τ' →
+      ∀ (l : ILit), (l ∈ C →
+        (τ'.litValue? l = some false) ∧
+        (τ.litValue? l = none → τ'.isSetFor (toVar l) = bumps + 1) ∧
+        (τ.litValue? l = some false → τ'.isSetFor (toVar l) = τ.isSetFor (toVar l))) ∧
+         (l ∉ C → (-l) ∉ C → τ'.litValue? l = τ.litValue? l ∧ τ'.isSetFor (toVar l) = τ.isSetFor (toVar l)) := by
+  have ⟨C⟩ := C
+  induction' C with l ls ih generalizing τ
+  · simp [← Array.mem_data]; rintro rfl l; exact ⟨rfl, rfl⟩
+  · intro h
+    have h_copy := h
+    simp [assumeNegatedClauseFor, ← Array.mem_data, -Array.size_mk] at h ⊢
+    simp [← Array.mem_data] at ih
+    intro l'
+    constructor
+    · rintro (rfl | hmem)
+      · split at h <;> rename litValue? τ l' = _ => heq
+        · by_cases hls : l' ∈ ls
+          · rcases (ih h l').1 hls with ⟨h₁, _, h₃⟩
+            simp at h₃
+            simp [heq]
+            exact ⟨h₁, h₃⟩
+          · by_cases hlsn : (-l') ∈ ls
+            · have : Clause.toPropFun ({ data := l' :: ls } : IClause) = ⊤ := by
+                rw [Clause.tautology_iff]
+                use l'
+                simp [← Array.mem_data] at hls ⊢
+                exact ⟨_, hlsn, by simp⟩
+              replace this : τ.toPropFun ≤ ({ data := l' :: ls } : IClause) := by
+                rw [this]; exact le_top
+              rcases assumeNegatedClauseFor_error_of_le bumps this with ⟨τ'', hτ''⟩
+              rw [hτ''] at h_copy
+              injection h_copy
+            · rcases (ih h l').2 hls hlsn with ⟨h₁, h₂⟩
+              simp at h₁ h₂
+              simp [heq]
+              exact ⟨h₁, h₂⟩
+        · by_cases hls : l' ∈ ls
+          · exact (ih h l').1 hls
+          · by_cases hlsn : (-l') ∈ ls
+            · have : Clause.toPropFun ({ data := l' :: ls } : IClause) = ⊤ := by
+                rw [Clause.tautology_iff]
+                use l'
+                simp [← Array.mem_data] at hls ⊢
+                exact ⟨_, hlsn, by simp⟩
+              replace this : τ.toPropFun ≤ ({ data := l' :: ls } : IClause) := by
+                rw [this]; exact le_top
+              rcases assumeNegatedClauseFor_error_of_le bumps this with ⟨τ'', hτ''⟩
+              rw [hτ''] at h_copy
+              injection h_copy
+            · rcases (ih h l').2 hls hlsn with ⟨h₁, h₂⟩
+              simp [heq] at h₁ ⊢
+              exact ⟨h₁, h₂⟩
+        · have : τ.toPropFun ≤ ({ data := l' :: ls } : IClause) := by
+            simp [le_sup_of_le_left (litValue?_true_iff.mp heq)]
+          rcases assumeNegatedClauseFor_error_of_le bumps this with ⟨τ'', hτ''⟩
+          rw [hτ''] at h_copy
+          injection h_copy
+      · split at h <;> rename litValue? τ l = _ => heq
+        · rcases (ih h l').1 hmem with ⟨h₁, h₂, h₃⟩
+          use h₁
+          rcases eq_trichotomy l l' with (rfl | rfl | hll')
+          · simp [heq] at h₃ ⊢
+            exact h₃
+          · have : Clause.toPropFun ({ data := -l' :: ls } : IClause) = ⊤ := by
+              rw [Clause.tautology_iff]
+              use l'
+              simp [← Array.mem_data]
+              exact hmem
+            replace this : τ.toPropFun ≤ ({ data := -l' :: ls } : IClause) := by
+              rw [this]; exact le_top
+            rcases assumeNegatedClauseFor_error_of_le bumps this with ⟨τ'', hτ''⟩
+            rw [hτ''] at h_copy
+            injection h_copy
+          · have : toVar (-l) ≠ toVar l' := by simp [hll']
+            rw [litValue?_setLitFor_of_ne this] at h₂ h₃
+            rw [setLitFor_isSetFor_of_ne this] at h₃
+            exact ⟨h₂, h₃⟩
+        · exact (ih h l').1 hmem
+        · injection h
+    · simp [not_or]
+      intro hne hmem h_neg_ne h_neg_mem
+      split at h <;> rename litValue? τ l = _ => heq
+      · rcases (ih h l').2 hmem h_neg_mem with ⟨h₁, h₂⟩
+        have : toVar (-l) ≠ toVar l' := by
+          rcases eq_trichotomy l l' with (rfl | rfl | h) <;> try contradiction
+          simp [h]
+        rw [litValue?_setLitFor_of_ne this] at h₁
+        rw [setLitFor_isSetFor_of_ne this] at h₂
+        exact ⟨h₁, h₂⟩
+      · exact (ih h l').2 hmem h_neg_mem
+      · injection h
+
+/-
+For a general statement, we might say something like:
+
+theorem assumeNegatedClauseFor_ok {τ τ' : PPA} {C : IClause} {bumps : Nat} :
+    (τ.assumeNegatedClauseFor C bumps) = .ok τ' →
+      ∀ (l : ILit), (l ∈ C →
+        (τ'.litValue? l = some false) ∧
+        (τ.litValue? l = none → τ'.isSetFor (toVar l) = bumps + 1) ∧
+        (τ.litValue? l = some false → τ'.isSetFor (toVar l) = τ.isSetFor (toVar l))) ∧
+         (l ∉ C → (-l) ∉ C → τ'.litValue? l = τ.litValue? l ∧ τ'.isSetFor (toVar l) = τ.isSetFor (toVar l))
+
+However, the SR checker only assumes the negated clause on a reset assignment.
+So we prove the specific case, which allows us to write `uniform` instead of
+the complicated expression above as a postcondition.
+-/
+
+-- Just to simplify things, we include the postcondition from aNCF_ok
+theorem assumeNegatedClauseFor_reset_ok {τ τ' : PPA} {C : IClause} {bumps : Nat} :
+  (τ.reset.assumeNegatedClauseFor C bumps) = .ok τ' →
+    τ'.toPropFun = (C.toPropFun)ᶜ ∧ uniform τ' bumps := by
+  intro h
+  have := assumeNegatedClauseFor_ok h
+  simp at this
+  rcases this with ⟨h₁, h₂⟩
+  exact ⟨h₁, uniform_of_extended_reset h₂⟩
+
+end assumeNegatedClause /- section -/
 
 /-! ## Tautology checking -/
 
@@ -882,33 +1283,21 @@ where
         have : (↑l)ᶜ ≤ C.toPropFun := by
           apply le_trans this
           rw [τ.property]
-          apply C.toPropFun_take_lt
-        have : l ≤ C.toPropFun := C.toPropFun_getElem_lt _
+          apply C.toPropFun_take_le
+        have : l ≤ C.toPropFun := C.toPropFun_getElem_le _
         have : ⊤ ≤ C.toPropFun := by
           rw [← sup_compl_eq_top (x := l.toPropFun)]
           apply sup_le <;> assumption
         simp only [top_le_iff.mp this]⟩)
     | some false =>
       go (i + 1) ⟨τ.val.setLit (-l), by
-        have := litValue?_negate τ.val l
-        rw [h, Option.map_some', Bool.not, Bool.not_false] at this
-        have := toPropFun_setLit_of_true this
-
-        rw [← litValue?_negate] at h
-        have : (τ.val.setLit (-l)).toPropFun ≤ τ.val.toPropFun := by
-          apply entails_ext.mpr
-          intro σ hσ
-          rw [satisfies_iff_vars] at hσ ⊢
-          intro x b hx
-          apply hσ
-          by_cases hEq : toVar (-l) = x
-          . aesop (add norm unfold litValue?, norm unfold setLit)
-          . rwa [τ.val.varValue?_setLit_of_ne hEq]
-        have := τ.val.toPropFun_setLit_lt (-l)
-        have : (τ.val.setLit (-l)).toPropFun = τ.val.toPropFun ⊓ (-l).toPropFun := by
-          refine le_antisymm ?_ (τ.val.lt_toPropFun_setLit _)
-          simp_all only [le_inf_iff, and_self]
-        simp [*, τ.property]⟩
+        rw [hCl]
+        conv => rhs; lhs; rw [← τ.property]
+        rw [← litValue?_negate_some_iff', Bool.not_false] at h
+        rw [toPropFun_setLit_of_true h]
+        rw [litValue?_negate_some_iff, Bool.not_true, litValue?_false_iff] at h
+        rw [left_eq_sup, ← compl_le_compl_iff_le, compl_compl]
+        exact h⟩
     | none =>
       go (i + 1) ⟨τ.val.setLit (-l), by
         have : (τ.val.setLit (-l)).toPropFun = τ.val.toPropFun ⊓ (-l).toPropFun := by
@@ -925,7 +1314,7 @@ where
       have that : C = { data := C.data } := rfl
       simp_rw [C.data.take_length_le this, ← that, h, compl_eq_top] at hEq
       assumption⟩)
-termination_by go i τ => C.size - i
+termination_by C.size - i
 
 /-! ## Unit propagation -/
 
@@ -1005,7 +1394,8 @@ where
           exfalso
           rcases (satisfies_conj.mp hσ) with ⟨hσC, hστ⟩
           have ⟨l, hl, hσl⟩ := Clause.satisfies_iff.mp hσC
-          have ⟨k, hk⟩ := Array.mem_data_iff.mp hl
+          rw [← Array.mem_data] at hl
+          have ⟨k, hk⟩ := Array.mem_data_iff_exists_fin.mp hl
           rw [not_lt] at hi
           have := hLits k (lt_of_lt_of_le k.is_lt hi)
           simp only [false_or] at this
@@ -1023,7 +1413,8 @@ where
             intro σ hσ
             have ⟨hστ, hσC⟩ := satisfies_conj.mp hσ
             have ⟨l, hl, hσl⟩ := Clause.satisfies_iff.mp hσC
-            have ⟨i, hi⟩ := Array.mem_data_iff.mp hl
+            rw [← Array.mem_data] at hl
+            have ⟨i, hi⟩ := Array.mem_data_iff_exists_fin.mp hl
             have := i.is_lt
             have := hLits i (by linarith)
             rcases this with hEq | hτl
@@ -1031,7 +1422,7 @@ where
               rwa [hi]
             . exfalso
               exact (satisfies_neg.mp <| entails_ext.mp hτl _ hστ) (hi ▸ hσl))⟩
-  termination_by go i _ _ _ => C.size - i
+  termination_by C.size - i
 
 -- Cayden's alternate implementation of unit propagation (TODO: Compare for efficiency)
 
@@ -1049,13 +1440,13 @@ inductive MUPDone where
   | satisfied
   | multipleUnassignedLiterals
 
-open ResultT MUPResult MUPDone
+open Except MUPResult MUPDone
 
-abbrev UPBox := ResultT MUPDone (Option ILit)
+abbrev UPBox := Except MUPDone (Option ILit)
 
 def pevalUP (τ : PPA) (unit? : Option ILit) (l : ILit) : UPBox :=
   match τ.litValue? l with
-  | some true => done .satisfied
+  | some true => error .satisfied
   | some false => ok unit?
   | none =>
     match unit? with
@@ -1063,7 +1454,7 @@ def pevalUP (τ : PPA) (unit? : Option ILit) (l : ILit) : UPBox :=
     | some u =>
       if u = l then ok unit?
       -- Assume tautology cannot occur in clause, so two unassiged literals exits early
-      else done .multipleUnassignedLiterals
+      else error .multipleUnassignedLiterals
 
 def foldUP (τ : PPA) (C : IClause) := C.foldlM (pevalUP τ) none
 
@@ -1071,8 +1462,8 @@ def unitProp (τ : PPA) (C : IClause) : MUPResult :=
   match foldUP τ C with
   | ok none => .falsified
   | ok (some lit) => .unit lit
-  | done .satisfied => .satisfied
-  | done .multipleUnassignedLiterals => .multipleUnassignedLiterals
+  | error .satisfied => .satisfied
+  | error .multipleUnassignedLiterals => .multipleUnassignedLiterals
 
 def motive_fn (τ : PPA) (C : IClause) : ℕ → Option ILit → Prop
   | idx, none => ∀ ⦃i : Fin C.size⦄, i < idx → τ.litValue? C[i] = some false
@@ -1090,7 +1481,7 @@ theorem SatisfiesM_UP (τ : PPA) (C : IClause) :
     (h0 := by simp [motive_fn]) -- Why do I have to define it right above? Putting it inline with (motive :=) had sorryAx problems
     (hf := by
       unfold motive_fn
-      simp only [SatisfiesM_ResultT_eq, getElem_fin]
+      simp only [SatisfiesM_Except_eq, getElem_fin]
       intro i box ih
         -- Cayden question: Is this proof more compact if I use pattern-matching with intro?
       intro
@@ -1122,7 +1513,7 @@ theorem SatisfiesM_UP (τ : PPA) (C : IClause) :
           | none =>
             subst h_box
             simp at hbox
-            use Array.mem_data_iff.mpr ⟨i, hbox⟩, hbox ▸ h_tau
+            use Array.mem_data_iff_exists_fin.mpr ⟨i, hbox⟩, hbox ▸ h_tau
             intro j hj₁ hj₂
             rcases lt_or_eq_of_le (le_of_lt_succ hj₁) with (h | h)
             · exact ih h
@@ -1156,14 +1547,14 @@ theorem SatisfiesM_UP (τ : PPA) (C : IClause) :
   intro
   | none =>
     intro h l hl
-    rcases Array.mem_data_iff.mp hl with ⟨i, rfl⟩
+    rcases Array.mem_data_iff_exists_fin.mp hl with ⟨i, rfl⟩
     exact h i.isLt
   | some lit =>
     simp [motive_fn]
     intro hlit₁ hlit₂ ih
     use hlit₁, hlit₂
     intro l hl₁ hl₂
-    rcases Array.mem_data_iff.mp hl₁ with ⟨i, rfl⟩
+    rcases Array.mem_data_iff_exists_fin.mp hl₁ with ⟨i, rfl⟩
     exact ih hl₂
 
 -- Cayden TODO/Q: Allow for [pattern_match] on ResultT? What is [unbox]?
@@ -1180,7 +1571,8 @@ theorem contradiction_of_UP_falsified {τ : PPA} {C : IClause} :
   rw [satisfies_conj] at hτ'
   rcases hτ' with ⟨hττ', hCτ'⟩
   have ⟨lit, hlit, hτ'lit⟩ := Clause.satisfies_iff.mp hCτ'
-  have hlv := SatisfiesM_ResultT_eq.mp (SatisfiesM_UP τ C) none h lit hlit
+  rw [← Array.mem_data] at hlit
+  have hlv := SatisfiesM_Except_eq.mp (SatisfiesM_UP τ C) none h lit hlit
   clear h hCτ' hlit
   have := satisfies_iff_vars.mp hττ'
   replace hτ'lit := LitVar.satisfies_iff.mp hτ'lit
@@ -1193,139 +1585,37 @@ theorem contradiction_of_UP_falsified {τ : PPA} {C : IClause} :
 -- Is it better to say that ¬(τ ≤ l), or that τ.litValue? l = none?
 theorem extended_of_UP_unit {τ : PPA} {C : IClause} {l : ILit} :
     τ.unitProp C = .unit l →
-      C.toPropFun ⊓ τ.toPropFun ≤ l.toPropFun
-      ∧ ¬(τ.toPropFun ≤ l.toPropFun) -- Cayden: see litValue?_none_iff
-      ∧ ¬(τ.toPropFun ≤ l.toPropFunᶜ) := by
+      l ∈ C ∧
+      τ.litValue? l = none ∧
+      C.toPropFun ⊓ τ.toPropFun ≤ l.toPropFun ⊓ τ := by
   unfold unitProp
   intro h_unit
   split at h_unit
   <;> try simp at h_unit
   rename ILit => lit; subst h_unit
   rename (foldUP τ C = ok (some lit)) => h
-  have hlv := SatisfiesM_ResultT_eq.mp (SatisfiesM_UP τ C) (some lit) h
+  have hlv := SatisfiesM_Except_eq.mp (SatisfiesM_UP τ C) (some lit) h
   clear h
   rcases hlv with ⟨hlit, hτlit, ih⟩
-  constructor
-  · refine entails_ext.mpr fun τ' hτ' => ?_
-    rw [satisfies_conj] at hτ'; rcases hτ' with ⟨hCτ', hττ'⟩
-    rw [satisfies_iff_lits] at hττ'
-    rw [Clause.satisfies_iff] at hCτ'; rcases hCτ' with ⟨m, hm, hmτ'⟩
-    by_cases heq : m = lit
-    · subst heq; exact hmτ'
-    · replace ih := ih _ hm heq
-      have := litValue?_negate τ m
-      simp only [ih, Option.map_some', Bool.not_false] at this
-      have := hττ' this
-      simp at this
-      exact absurd hmτ' this
-  · exact litValue?_none_iff.mp hτlit
+  rw [← Array.mem_data]
+  use hlit, hτlit
+  refine entails_ext.mpr fun τ' hτ' => ?_
+  rw [satisfies_conj] at hτ'; rcases hτ' with ⟨hCτ', hττ'⟩
+  rw [satisfies_iff_lits] at hττ'
+  rw [Clause.satisfies_iff] at hCτ'; rcases hCτ' with ⟨m, hm, hmτ'⟩
+  by_cases heq : m = lit
+  · subst heq
+    rw [← satisfies_iff_lits] at hττ'
+    rw [satisfies_conj]
+    exact ⟨hmτ', hττ'⟩
+  · rw [← Array.mem_data] at hm
+    replace ih := ih _ hm heq
+    have := litValue?_negate τ m
+    simp only [ih, Option.map_some', Bool.not_false] at this
+    have := hττ' this
+    simp at this
+    exact absurd hmτ' this
 
-#exit
-
-/-
-theorem SatisfiesM_foldUPs (τ : PPA) (L : Array IClause) :
-    SatisfiesM (fun τ' => (clauses_to_PropFun L) ⊓ τ ≤ τ') (foldUPs τ L) := by
-  have := L.SatisfiesM_foldlM (init := (τ : PPA)) (f := applyUPHint)
-    (motive := fun idx τ' => (clauses_to_PropFun (L.take idx)) ⊓ τ ≤ τ')
-  done
--/
-
-/-
-def motive_fn (τ : PPA) (C : IClause) : ℕ → Option ILit → Prop
-  | idx, none => ∀ ⦃i : Fin C.size⦄, i < idx → τ.litValue? C[i] = some false
-  | idx, some lit => lit ∈ C.data ∧ τ.litValue? lit = none ∧
-      (∀ ⦃j : Fin C.size⦄, j < idx → C[j] ≠ lit → τ.litValue? C[j] = some false)
-
-    SatisfiesM (fun
-      -- If there are no unassigned literals, then all should be false
-      | none => ∀ l ∈ C.data, τ.litValue? l = some false
-      | some lit => lit ∈ C.data ∧ τ.litValue? lit = none ∧
-          (∀ l ∈ C.data, l ≠ lit → τ.litValue? l = some false)) (foldUP τ C) := by
-  have := C.SatisfiesM_foldlM (init := (none : Option ILit)) (f := pevalUP τ)
-    (motive := motive_fn τ C)
-    (h0 := by simp [motive_fn])
--/
-
-theorem SatisfiesM_foldUPs (τ : PPA) (L : Array IClause) :
-    SatisfiesM (fun τ' => (clauses_to_PropFun L) ⊓ τ ≤ τ') (foldUPs τ L) := by
-  have := L.SatisfiesM_foldlM (init := (τ : PPA)) (f := applyUPHint)
-    (motive := fun idx τ' => ∀ ⦃i : Fin L.size⦄, i < idx → L[i].toPropFun ⊓ τ ≤ τ')
-    (h0 := by
-      sorry
-      done)
-    (hf := by
-      sorry
-      done)
-  done
-
-#exit
-
-theorem foldUPs_correct {τ : PPA} {L : List IClause} :
-    foldUPs τ L = done true → (clauses_to_PropFun L) ⊓ τ = ⊥ := by
-  induction' L with C CS ih generalizing τ
-  · simp [foldUPs]
-  · intro h_UP
-    rw [foldUPs] at h_UP
-    rw [List.foldlM_eq_foldl] at h_UP
-    simp at h_UP
-
-    --simp [List.foldlM_cons, applyUPHint] at h_UP
-    --split at h_UP <;> try simp at h_UP
-
-    done
-  done
-
-#exit
-
-theorem unit_of_foldUPs_cons_ok {τ τ' : PPA} {C : IClause} {L : List IClause} :
-    foldUPs τ (C :: L) = ok τ' → ∃ (l : ILit) (τ'' : PPA), τ.unitProp C = unit l τ'' := by
-  intro h
-  rw [foldUPs, List.foldlM_cons, applyUPHint] at h
-  cases hτ : τ.unitProp C <;> simp [hτ] at h <;> try contradiction
-  exact ⟨_, _, rfl⟩
-
-theorem foldUPs_cons_of_falsified {τ : PPA} {C : IClause} {L : List IClause} :
-    τ.unitProp C = .falsified → foldUPs τ (C :: L) = done true := by
-  intro h; simp [foldUPs, List.foldlM_cons, applyUPHint, h]; rfl
-
-theorem foldUPs_ok {τ τ' : PPA} {L : List IClause} :
-    foldUPs τ L = ok τ' → (clauses_to_PropFun L) ⊓ τ ≤ τ' := by
-  induction' L with C CS ih generalizing τ
-  · simp; rintro rfl; exact Eq.ge rfl
-  · intro h
-    rw [clauses_to_PropFun_cons, inf_comm, ← inf_assoc, inf_comm]
-    rcases unit_of_foldUPs_cons_ok h with ⟨l, σ, hτ⟩
-    rw [foldUPs_cons_of_unit hτ] at h
-    apply le_trans _ (ih h)
-    have := (extended_of_UP_unit hτ).1
-    rw [inf_comm] at this
-    exact inf_le_inf_left _ this
-
-theorem foldUPs_true {τ : PPA} {L : List IClause} :
-    foldUPs τ L = done true → (clauses_to_PropFun L) ⊓ τ ≤ ⊥ := by
-  induction' L with C CS ih generalizing τ
-  · simp
-  · intro h
-    rw [foldUPs, List.foldlM_cons, applyUPHint] at h
-    split at h <;> try injection h <;> try contradiction
-    · rename unitProp τ C = falsified => heq
-      rw [clauses_to_PropFun_cons, inf_comm, ← inf_assoc]
-      exact le_trans inf_le_left (contradiction_of_UP_falsified heq)
-    · rename ILit => l
-      rename PPA => τ'
-      rename unitProp τ C = unit _ _ => heq
-      have := (extended_of_UP_unit heq).1
-      rw [inf_comm] at this
-      rw [clauses_to_PropFun_cons, inf_comm, ← inf_assoc, inf_comm]
-      apply le_trans (inf_le_inf_left (clauses_to_PropFun CS) this)
-      apply ih
-      rw [← h]
-      rfl
-
-#exit
-    --(clauses_to_PropFun (C :: L)) ⊓ τ = ⊥ := by
-
-
-end monadic
+end monadic /- section -/
 
 end PPA
