Experiments/ProofChecking/SRChecker.lean
@@ -7,22 +7,23 @@ Carnegie Mellon University
 
 -/
 
+import Experiments.ProofChecking.PPA
+import Experiments.ProofChecking.PS
+
 import LeanSAT.Data.Cnf
 import LeanSAT.Data.ICnf
-import LeanSAT.Data.PPA
-import LeanSAT.Data.PS
 import LeanSAT.Model.PropFun
-import LeanSAT.Model.Quantification
+import LeanSAT.Model.Subst
 
 namespace SR
 
 open LeanSAT LeanSAT.Model Nat
 open PPA PS LitVar ILit IVar LawfulLitVar PropFun
-open ResultT
+open Except
 
 inductive UPResult
   | checked : UPResult
-  | error : UPResult
+  | checkError : UPResult
 
 open UPResult
 
@@ -30,472 +31,156 @@ structure SRLine where
   clause : IClause
   witness_lits : Array ILit
   witness_maps : Array (IVar × ILit)
-  up_hints : Array Nat
-  rat_hints : Array (Nat × Array Nat)
+  up_hints : Array Nat                -- Already 0-indexed clause IDs into the accumulated formula
+  rat_hints : Array (Nat × Array Nat) -- Already 0-indexed clause IDs into the accumulated formula
 
 structure SRState where
-  F : ICnf
-  τ : PPA
-  σ : PS
+  F : ICnf -- Accumulated formula
+  τ : PPA  -- Partial assignment, to store candidate and RAT negations
+  σ : PS   -- Substitution, for the witness
 
--- Build τ from candidate redundant clause C. Resets from previous line.
-def assumeNegatedClause (τ : PPA) (C : IClause) (offset : Nat) : PPA :=
-  τ.reset.setNegatedClauseFor C offset
-
-/-
-theorem toPropFun_data_cons (l : L) (ls : List L) :
-    toPropFun ({ data := (l :: ls) } : Clause L) = LitVar.toPropFun l ⊔ toPropFun ( { data := ls } : Clause L) := by
-  rw [of_cons]; simp
--/
-
-@[simp] theorem assumeNegatedClause_empty (τ : PPA) (offset : Nat) :
-    assumeNegatedClause τ #[] offset = τ.reset := by
-  simp [assumeNegatedClause]
-  done
-
-#exit
-
-def applyUPHint (F : ICnf) (offset : Nat) (τ : PPA) (hint : Nat) : ResultT (PPA × UPResult) PPA :=
+-- Applies a single unit propagation step
+-- On success, we set the unit literal in τ with the offset
+-- On falsification of the clause, we error with .checked
+-- On satisfied clause or multiple unassigned literals, we error with checkError
+def applyUPHint (F : ICnf) (offset : Nat) (τ : PPA) (hint : Nat) : Except (PPA × UPResult) PPA :=
   if h_hint : hint < F.size then
     let C := F.get ⟨hint, h_hint⟩
     match τ.unitProp C with
-    | .falsified => done ⟨τ, .checked⟩
-    | .satisfied => done ⟨τ, .error⟩
-    | .multipleUnassignedLiterals => done ⟨τ, .error⟩
+    | .falsified => error ⟨τ, .checked⟩
+    | .satisfied => error ⟨τ, .checkError⟩
+    | .multipleUnassignedLiterals => error ⟨τ, .checkError⟩
     | .unit l => ok (τ.setLitFor l offset)
   else
-    done ⟨τ, .error⟩
+    error ⟨τ, .checkError⟩
 
--- Cayden TODO: Way to combine this along with reduced? in the non-up-next-RAT clause case?
--- Returns true if (C|σ) is satisfied by τ, false otherwise
-def evalsToTrueUnderWitness (C : IClause) (σ : PS) (τ : PPA) : Bool :=
-  match C.foldlM (init := ()) (fun _ lit =>
-    match σ.litValue lit with
-    | .tr => done ()   -- Shouldn't get here
-    | .fls => ok ()
-    | .lit l =>
-      match τ.litValue? l with
-      | some true => done () -- τ satisfies the clause C, so we're done
-      | some false => ok ()
-      | none => ok ()) with
-  | ok () => false
-  | done () => true
+def scanRATHints (clauseId : Nat) (ratHints : Array (Nat × Array Nat)) : Option (Fin ratHints.size) :=
+  match ratHints.foldlM (init := 0) (fun counter ⟨hint, _⟩ =>
+        if hint = clauseId then error counter
+        else ok (counter + 1)) with
+  | ok _ => none
+  | error index =>
+    if hi : index < ratHints.size then some ⟨index, hi⟩
+    else none
+
+-- Finds the RAT hint pair that matches the clauseId
+def findRATHintIndex (ratIndex clauseId : Nat) (ratHints : Array (Nat × Array Nat)) : Option (Fin ratHints.size) :=
+  -- If the RAT hints are sorted, then check the one under our "cached pointer" first
+  if h_index : ratIndex < ratHints.size then
+    let ⟨ratClauseIndex, _⟩ := ratHints.get ⟨ratIndex, h_index⟩
+    if ratClauseIndex = clauseId then some ⟨ratIndex, h_index⟩
+    else scanRATHints clauseId ratHints
+  else
+    scanRATHints clauseId ratHints
 
 -- Assuming that (C|σ) is reduced but not satisfied and that C is a RAT clause, sets τ ← τ ⊓ (C|σ)ᶜ
-def assumeRATClause (C : IClause) (σ : PS) (τ : PPA) : ResultT Unit PPA :=
+def assumeRATClause (C : IClause) (σ : PS) (τ : PPA) : Except PPA PPA :=
   C.foldlM (init := τ) (fun τ lit =>
     match σ.litValue lit with
-    | .tr => done ()      -- (C|σ) isn't satisfied, so we shouldn't get here
-    | .fls => ok τ        -- Ignore the literal
+    | .tr => error τ       -- (C|σ) is satisfied, so return early to report satisfied
+    | .fls => ok τ         -- Ignore the literal
     | .lit l =>
       match τ.litValue? l with
-      | some true => done ()   -- (C|σ)|τ is satisfied, so we're done (shouldn't happen)
-      | some false => ok τ     -- Its negation is true in τ, so ignore the literal
+      | some true => error τ    -- (C|σ)|τ is satisfied, so return early to report satisfied
+      | some false => ok τ      -- Its negation is true in τ, so ignore the literal
       | none => ok (τ.setLit (-l)))
 
 -- Set the witness substitution σ from the provided mapping, resetting σ first
-def assumeWitness (σ : PS) (A₁ : Array ILit) (A₂ : Array (IVar × ILit)) : PS :=
-  (A₁.foldl (init := σ.reset) (fun σ' l => σ'.setLit l)).setVars' A₂
+def assumeWitness (σ : PS) (pivot : ILit) (A₁ : Array ILit) (A₂ : Array (IVar × ILit)) : PS :=
+  ((σ.reset.setLits A₁).setVars A₂).setLit pivot
 
+-- Check each clause in the formula.
+-- C is the current clause in the formula to be checked for the RAT property under σ and τ
+-- If C is reduced by σ, then it is RAT. Find a RAT hint and uses the RAT UP hints to derive contradiction.
 def checkClause (F : ICnf) (σ : PS) (ratHints : Array (Nat × Array Nat))
-    (p : PPA × Nat) (index : Fin F.size) (C : IClause) : ResultT Unit (PPA × Nat) :=
-  let ⟨τ, ratIndex⟩ := p
+    (p : PPA × Nat × Nat × Nat) (C : IClause) : Except Unit (PPA × Nat × Nat × Nat) :=
+  let ⟨τ, ratIndex, index, bumpCounter⟩ := p
   match σ.reduce C with
-  | .satisfied => ok (τ, ratIndex)
-  | .notReduced => ok (τ, ratIndex)
+  | .satisfied => ok (τ, ratIndex, index + 1, bumpCounter)
+  | .notReduced => ok (τ, ratIndex, index + 1, bumpCounter)
   | _ =>
-    -- The clause was reduced but not satisfied, so we have a candidate RAT clause
-    -- If the clause index doesn't match the current index, then the proof doesn't check
-    if h_index : ratIndex < ratHints.size then
-      let ⟨ratClauseIndex, ratClauseHints⟩ := ratHints.get ⟨ratIndex, h_index⟩
-      if index.val != ratClauseIndex then
-        -- The potential RAT clause can be satisfied by τ instead, so check that. If not, error.
-        if evalsToTrueUnderWitness C σ τ then
-          ok (τ, ratIndex)
-        else
-          done ()
-      else
-        match assumeRATClause C σ τ with
-        -- If we early exit from assumeRATClause, then the RAT clause trivially checks
-        | done _ => ok (τ.bump, ratIndex + 1)
-        | ok τ =>
-          match ratClauseHints.foldlM (init := τ) (applyUPHint F 0) with
-          | done (τ, .checked) => ok (τ.bump, ratIndex + 1)
-          | done (_, .error) => done ()
-          -- We expect contradiction at the end of the hints
-          | ok _ => done ()
-    else
-      done ()
+    -- We expect a RAT clause. Check if we have bumps left
+    if bumpCounter < ratHints.size then
+      -- Curiously, if the clause is completely falsified, we can still succeed
+      -- on the check (which sr-check does not allow). This is because a UP
+      -- derivation on a completely falsified clause is a global UP derivation,
+      -- and so the certificate can be reduced quite a bit.
 
-def checkLine (S : SRState) (line : SRLine) : ResultT Bool SRState :=
+      -- Find a RAT hint matching the clause
+      -- We hope that the hints are sorted, but they don't have to be
+      match findRATHintIndex ratIndex (index + 1) ratHints with
+      | none => error ()
+      | some rI =>
+        let ⟨_, hints⟩ := ratHints.get rI
+        match assumeRATClause C σ τ with
+        -- If the clause is satisfied under σ and τ, then we move to the next iteration
+        | error τ => ok (τ.bump, rI.val + 1, index + 1, bumpCounter + 1)
+
+        -- Otherwise, we have assumed the negation of the RAT clause
+        -- Now check for UP derivation through its hints
+        | ok τ =>
+          match hints.foldlM (init := τ) (applyUPHint F 0) with
+          | error (τ, .checked) => ok (τ.bump, rI.val + 1, index + 1, bumpCounter + 1)
+          | error (_, .checkError) => error ()
+          | ok _ => error ()
+    -- We error if the bumpCounter equals the number of RAT hints, since that
+    -- means we bumped the assignment too many times, clearing out the
+    -- assumption of the candidate clause
+    else error ()
+
+def checkLine (S : SRState) (line : SRLine) : Except Bool SRState :=
   let ⟨F, τ, σ⟩ := S
   let ⟨C, w_tf, w_maps, UPhints, RAThints⟩ := line
-  let τ := assumeNegatedClause τ.reset C RAThints.size
 
-  -- Evaluate the UP hints
-  match UPhints.foldlM (init := τ) (applyUPHint F RAThints.size) with
-  | done ⟨τ, .checked⟩ =>
-    if C = #[] then
-      done true
-    else
-      ok ⟨F.addClause C, τ, σ⟩
-  | done ⟨_, .error⟩ => done false
-  -- Unit propagation didn't lead to contradiction, so continue
+  -- Assumes the negation of the candidate clause, with "# of RAT hints" offset
+  match assumeNegatedClauseFor τ.reset C (RAThints.size + 1) with
+  | error _ => error false
   | ok τ =>
 
-  -- Now add the witness (unless C is empty, at which point we error)
-  if C = #[] then done false else
-  if C.get? 0 ≠ w_tf.get? 0 then done false else
-  let σ := assumeWitness σ w_tf w_maps
+  -- Evaluate the UP hints, with "# of RAT hints" offset
+  -- We add one more than normal to help with proving
+  match UPhints.foldlM (init := τ) (applyUPHint F (RAThints.size + 1)) with
+  -- The clause led to contradiction via unit propagation
+  | error ⟨τ, .checked⟩ =>
+    if C = #[] then error true       -- If the clause is empty, we have a successful proof
+    else ok ⟨F.addClause C, τ, σ⟩ -- The clause is redundant, so add it to the formula
 
+  -- Unit propagation failed due to multiple unassigned literals, satisfied clause, or out-of-bounds
+  | error ⟨_, _⟩ => error false
 
-  -- Go through each clause in the formula. If the witness reduces it, but
-  -- doesn't satisfy it, try the next RAT hint
-  match F.foldlIdxM (init := (⟨τ, 0⟩ : PPA × Nat)) (checkClause F σ RAThints) with
-  | done () => done false
-  | ok (τ, _) => ok ⟨F.addClause C, τ, σ⟩ -- The RAT hint checked, so we continue
+  -- Unit propagation worked but didn't lead to contradiction, so continue to RAT checking
+  | ok τ =>
+
+    -- If the clause is empty, then we should have derived UP contradiction by now
+    if hCw : 0 < C.size ∧ 0 < w_tf.size then
+      if C.get ⟨0, hCw.1⟩ ≠ w_tf.get ⟨0, hCw.2⟩ then error false else
+
+      -- Assume the witness, under substitution (the function call resets σ)
+      let σ := assumeWitness σ (C.get ⟨0, hCw.1⟩) w_tf w_maps
+
+      -- Go through each clause in the formula to check RAT
+      match F.foldlM (init := (⟨τ, 0, 0, 0⟩ : PPA × Nat × Nat × Nat)) (checkClause F σ RAThints) with
+      | error () => error false
+      | ok (τ, _) => ok ⟨F.addClause C, τ, σ⟩ -- The RAT hint checked, so we continue
+
+    else error false
 
 def checkProof (F : ICnf) (proof : Array SRLine) : Bool :=
   let τ := PPA.new 100
   let σ := PS.new 100
   match proof.foldlM (init := ⟨F, τ, σ⟩) checkLine with
   | ok _ => false
-  | done false => false
-  | done true => true
-
------------------------------------------
+  | error false => false
+  | error true => true
 
 /-! # correctness -/
 
-theorem applyUPHint_checked {F : ICnf} {offset : Nat} {τ : PPA} {hint : Nat} :
-    applyUPHint F offset τ hint = .done (τ, .checked) → F.toPropFun ⊓ τ ≤ ⊥ := by
-  intro h
-  unfold applyUPHint at h
-  split at h <;> simp at h
-  split at h <;> simp at h
-  rename hint < F.size => h_hint
-  rename (unitProp τ _ = _) => h_up
-  have := contradiction_of_UP_falsified h_up
-  rw [inf_comm] at this
-  have h_le : F.toPropFun ≤ F[hint].toPropFun := Cnf.ith_le ⟨hint, h_hint⟩
-  exact le_trans (inf_le_inf_right τ.toPropFun h_le) this
-
-theorem applyUPHint_checked_eq {F : ICnf} {offset : Nat} {τ τ' : PPA} {hint : Nat} :
-    applyUPHint F offset τ hint = .done (τ', .checked) → τ = τ' := by
-  sorry
-  done
-
-theorem applyUPHint_ok {F : ICnf} {offset : Nat} {τ τ' : PPA} {hint : Nat} :
-    applyUPHint F offset τ hint = .ok τ' → F.toPropFun ⊓ τ ≤ τ' := by
-  intro h
-  unfold applyUPHint at h
-  split at h <;> simp at h
-  split at h <;> simp at h
-  rename hint < F.size => h_hint
-  rename (unitProp τ _ = _) => h_up
-  subst h
-  have := (extended_of_UP_unit h_up).1
-  simp at this
-  sorry
-  --exact le_trans (inf_le_inf_right τ.toPropFun (Cnf.ith_le ⟨hint, h_hint⟩)) this
-
-#check Array.foldl
-
-theorem assumeNegatedClause_spec (τ : PPA) (C : IClause) (offset : Nat) :
-    (assumeNegatedClause τ C offset).toPropFun = C.toPropFunᶜ ∧
-    ∀ l ∈ C, τ.isSetFor (toVar l) (offset + 1) := by
-  have ⟨C⟩ := C
-  rw [assumeNegatedClause]
-  induction' C with l ls ih generalizing τ
-  · simp [setNegatedClauseFor]
-  · simp only [setNegatedClauseFor, Array.size_mk, List.length_cons, Clause.toPropFun_data_cons,
-    compl_sup]
-    done
-  sorry
-  done
-
-#exit
-
-open Classical
--- TODO: How to write the spec for this?
--- Jeremy: Can write the computational version of this, but if it's only for a theorem,
---         no need to make this efficient
-theorem assumeWitness_spec (σ : PS) (A₁ : Array ILit) (A₂ : Array (IVar × ILit)) :
-    (assumeWitness σ A₁ A₂).toSubst =
-      (fun v => if ∃ (l : ILit), (v, l) ∈ A₂ then l
-        else if ∃ l ∈ A₁, (toVar l) = v then
-          if isPos l then ⊤ else ⊥
-        else v.toPropFun) := by
-  sorry
-  done
-
-#exit
-
-theorem fold_UP_checked {F : ICnf} {A : Array Nat} {offset : Nat} {τ τ' : PPA} :
-    A.foldlM (init := τ) (applyUPHint F offset) = done (τ', .checked) →
-    F.toPropFun ⊓ τ ≤ ⊥ := by
-  have ⟨A⟩ := A
-  rw [Array.foldlM_eq_foldlM_data]
-  induction' A with n ns ih generalizing τ
-  · simp
-  · simp
-    intro h
-    match hn : applyUPHint F offset τ n with
-    | done (τ₁, .checked) =>
-      rw [← applyUPHint_checked_eq hn] at hn
-      exact le_bot_iff.mp (applyUPHint_checked hn)
-    | done (τ₁, .error) =>
-      simp [hn] at h; injection h
-      rename _ => h
-      simp at h
-      done
-    | ok τ₁ =>
-      simp [hn] at h
-      have := ih h
-      have := inf_le_inf_left F.toPropFun (applyUPHint_ok hn)
-      rw [← inf_assoc, inf_idem] at this
-      exact le_bot_iff.mp (le_trans this (ih h))
-
-theorem fold_UP_ok {F : ICnf} {A : Array Nat} {offset : Nat} {τ τ' : PPA} :
-    A.foldlM (init := τ) (applyUPHint F offset) = ok τ' →
-    F.toPropFun ⊓ τ ≤ τ' := by
-  have ⟨A⟩ := A
-  rw [Array.foldlM_eq_foldlM_data]
-  induction' A with n ns ih generalizing τ
-  · simp [pure]; rintro rfl; exact inf_le_right
-  · simp
-    intro h
-    match hn : applyUPHint F offset τ n with
-    | done (τ₁, .error)   => simp [hn] at h; injection h
-    | done (τ₁, .checked) => simp [hn] at h; injection h
-    | ok τ₁ =>
-      simp [hn] at h
-      have := ih h
-      have := inf_le_inf_left F.toPropFun (applyUPHint_ok hn)
-      rw [← inf_assoc, inf_idem] at this
-      exact le_trans this (ih h)
-
---τ.toPropFun ≤ (PropFun.bind σ.toSubst C.toPropFun) ∧
--- TODO: Hypotheses about form of τ' wrt τ and SetFor judgment
-theorem assumeRATClause_ok {C : IClause} {σ : PS} {τ τ' : PPA} :
-    (PropFun.bind σ.toSubst C.toPropFun ≠ ⊤) →
-    assumeRATClause C σ τ = ok τ' →
-    τ'.toPropFun = τ.toPropFun ⊓ (PropFun.bind σ.toSubst C.toPropFun)ᶜ := by
-  have ⟨C⟩ := C
-  intro h_notSatisfied h
-  rw [assumeRATClause, Array.foldlM_eq_foldlM_data] at h
-  induction' C with l ls ih generalizing τ
-  · rw [List.foldlM_nil] at h; injection h with h; subst h; simp
-  · simp at h h_notSatisfied ⊢
-    split at h <;> rename litValue _ _ = _ => hl <;> try simp [ResultT.bind, Bind.bind] at h
-    · rw [litValue_fls_iff] at hl; simp [hl]
-      apply ih (ne_top_right_of_disj_ne_top h_notSatisfied)
-      rw [h]
-    · rename ILit => lit
-      split at h <;> try simp at h
-      rename PPA => τ''
-      rename _ = ok τ'' => h₁
-      rw [litValue_lit_iff] at hl; simp [hl]
-      have := @ih τ'' (ne_top_right_of_disj_ne_top h_notSatisfied)
-      simp [h] at this
-      split at h₁ <;> rename litValue? _ _ = _ => hlit <;> try simp at h₁
-      · subst h₁
-        rwa [← inf_assoc, inf_eq_of_litValue?_false hlit]
-      · subst h₁
-        rw [litValue?_none_iff_litValue?_negate_none] at hlit
-        rwa [toPropFun_setLit_of_none hlit, toPropFun_neg, inf_assoc] at this
-
-theorem assumeRATClause_done {C : IClause} {σ : PS} {τ : PPA} :
-    (PropFun.bind σ.toSubst C.toPropFun ≠ ⊤) →
-    assumeRATClause C σ τ = done () → τ.toPropFun ≤ (PropFun.bind σ.toSubst C.toPropFun) := by
-  sorry
-  done
-
-/-
-  have ⟨C⟩ := C
-  intro h_notSatisfied h
-  rw [assumeRATClause, Array.foldlM_eq_foldlM_data] at h
-  induction' C with l ls ih generalizing τ
-  · simp at h
-  · split at h <;> try simp at h
-    subst h; rename PPA => τ'; rename _ => ih
-    rename List.foldlM _ _ _ = _ => h
-    rw [Clause.toPropFun, List.foldr_cons, ← Clause.toPropFun, bind_disj] at h_notSatisfied
-    rw [Clause.toPropFun, List.foldr_cons, ← Clause.toPropFun]
-    have := Ne.lt_of_le h_notSatisfied le_top
-    replace this := lt_of_le_of_lt le_sup_right this
-    replace this := LT.lt.ne this
-    simp at h
-    split at h <;> rename litValue _ _ = _ => hl
-    · rw [litValue_tr_iff] at hl; simp [hl] at h_notSatisfied
-    · rw [litValue_fls_iff] at hl; simp [hl]
-      replace ih := @ih τ this
-      simp [ResultT.bind, Bind.bind] at h
-      simp [h] at ih
-      exact ih
-    · rename ILit => lit
-      rename PSVal => val
-      rw [litValue_lit_iff] at hl; simp [hl]
-      split at h <;> rename litValue? _ _ = _ => hlit
-      · injection h with h; subst h
-        rw [litValue?_true_iff] at hlit
-
-        exact le_sup_of_le_left hlit
-      · simp [ResultT.bind, Bind.bind] at h
-        replace ih := @ih τ this
-        simp [h] at ih
-        exact le_sup_of_le_right ih
-      · replace ih := @ih (τ.setLit (-lit)) this
-        simp [ResultT.bind, Bind.bind] at h
-        simp [h] at ih
-        have hlit' : τ.litValue? (-lit) = none := by
-          rw [litValue?_negate, hlit]; rfl
-        rw [toPropFun_setLit_of_none hlit'] at ih
-        rw [toPropFun_neg, helper, compl_compl] at ih
-        exact ih -/
-
-
-theorem evalsToTrueUnderWitness_true {C : IClause} {σ : PS} {τ : PPA} :
-    (PropFun.bind σ.toSubst C.toPropFun ≠ ⊤) →
-    evalsToTrueUnderWitness C σ τ = true →
-    τ.toPropFun ≤ (PropFun.bind σ.toSubst C.toPropFun) := by
-  have ⟨C⟩ := C
-  intro h_notSatisfied
-  rw [evalsToTrueUnderWitness, Array.foldlM_eq_foldlM_data]
-  induction' C with l ls ih <;> simp
-  intro h
-  split at h <;> try contradiction
-  rename _ => h; clear h
-  rename _ => h
-  simp at h_notSatisfied
-  have := Ne.lt_of_le h_notSatisfied le_top
-  replace this := lt_of_le_of_lt le_sup_right this
-  replace this := LT.lt.ne this
-  split at h <;> rename litValue _ _ = _ => hl
-  · rw [litValue_tr_iff] at hl; simp [hl]
-  · rw [litValue_fls_iff] at hl; simp [hl]
-    simp [ResultT.bind, Bind.bind] at h
-    apply ih this
-    rw [h]
-  · rename ILit => lit
-    rename PSVal => val
-    rw [litValue_lit_iff] at hl; simp [hl]
-    split at h <;> rename litValue? _ _ = _ => hlit
-    · rw [litValue?_true_iff] at hlit
-      exact le_sup_of_le_left hlit
-    -- Cayden TODO: These two proofs are duplicated
-    · simp [ResultT.bind, Bind.bind] at h
-      have := ih this
-      simp [h] at this
-      exact le_sup_of_le_right this
-    · simp [ResultT.bind, Bind.bind] at h
-      have := ih this
-      simp [h] at this
-      exact le_sup_of_le_right this
-
-/-
-theorem comps_eq_of_checkClause_ok_ratIndex {F : ICnf} {σ : PS} {rat_hints : Array (Nat × Array Nat)}
-    {τ τ' β β' : PPA} {ratIndex : Nat} {index : Fin F.size} {C : IClause} :
-    checkClause F σ rat_hints τ β ratIndex index
-
-theorem ok_eq_of_checkClause_ok {F : ICnf} {σ : PS} {rat_hints : Array (Nat × Array Nat)}
-    {τ τ' β β' : PPA} {ratIndex : Nat} {index : Fin F.size} {C : IClause} :
-    checkClause F σ rat_hints τ β ratIndex index C = ok (τ', β', ratIndex) -/
-
-theorem checkClause_ok {F : ICnf} {σ : PS} {ratHints : Array (Nat × Array Nat)}
-    {τ τ' β β' : PPA} {ratIndex ratIndex' : Nat} {index : Fin F.size} {C : IClause} :
-    F[index.1] = C →
-    checkClause F σ ratHints ⟨τ, β, ratIndex⟩ index C = ok (τ', β', ratIndex') →
-      (PropFun.bind σ.toSubst C.toPropFun) = ⊥ ∨
-      F.toPropFun ⊓ τ ≤ PropFun.bind σ.toSubst C.toPropFun := by
-  intro hFC h
-  rw [checkClause] at h
-  match hσC : σ.reduced? β C with
-  | (.satisfied, _) => rw [reduced?_satisfied_iff] at hσC; simp [hσC]
-  | (.notReduced, _) =>
-    rw [reduced?_notReduced_iff] at hσC
-    rw [hσC]
-    -- Cayden TODO: What is the right kind of "mem" we should use here?
-    have := F.getElem_mem_data index.isLt
-    rw [hFC, Array.mem_data] at this
-    exact Or.inr (le_trans inf_le_left (Cnf.toPropFun_le_mem this))
-  | (.falsified, _) => rw [reduced?_falsified_iff, le_bot_iff] at hσC; simp [hσC]
-  | (.reduced, β₂) =>
-    right
-    simp [hσC] at h
-    replace hσC := reduced?_reduced hσC
-    split at h <;> try contradiction
-    -- Split into RAT clause/attempt to satisfy candidate RAT clause cases
-    rename ratIndex < _ => hri
-    split at h
-      -- Actual RAT clause case
-    · rename index.val = _ => hi
-      split at h <;> rename assumeRATClause _ _ _ = _ => h_assume
-      · exact le_trans inf_le_right (assumeRATClause_done hσC.1 h_assume)
-      · rename PPA => τ₂
-        have := assumeRATClause_ok hσC.1 h_assume
-        split at h <;> rename Array.foldlM _ _ _ = _ => h_fold <;> try contradiction
-        have := fold_UP_checked h_fold
-        rwa [assumeRATClause_ok hσC.1 h_assume, ← inf_assoc, ← le_iff_inf_compl_le_bot] at this
-        done
-      -- Candidate RAT clause case, to satisfy
-    · split at h
-      · rename evalsToTrueUnderWitness _ _ _ = _ => h_eval
-        exact le_trans inf_le_right (evalsToTrueUnderWitness_true hσC.1 h_eval)
-      · contradiction
-
---  match F.foldlIdxM (init := (⟨τ, β, 0⟩ : PPA × PPA × Nat)) (checkClause F σ RAThints)
-theorem fold_checkClause_ok {F : ICnf} {σ : PS} {ratHints : Array (Nat × Array Nat)}
-    {τ τ' β β' : PPA} {ratIndex : Nat} :
-    F.foldlIdxM (init := ⟨τ, β, 0⟩) (checkClause F σ ratHints) = ok (τ, β, ratIndex) →
-      F.toPropFun ⊓ τ ≤ (PropFun.bind σ.toSubst F) := by
-  have ⟨F⟩ := F
-  simp [Array.foldlIdxM, pure, Bind.bind, ResultT.bind]
-  rw [Array.foldlM_eq_foldlM_data]
-  induction' F with C CS ih generalizing τ β ratIndex <;> simp
-  intro h
-  split at h <;> try contradiction
-  rename (PPA × PPA × Nat) × Nat => acc
-  rename _ = ok acc => heq
-  simp at h
-  split at heq <;> try contradiction
-  rename (PPA × PPA × Nat) => acc'
-  rename _ = ok acc' => h_check
-  simp [h_check] at heq
-  simp [Cnf.of_cons]
-  have ⟨τ₂, β₂, ratIndex₂⟩ := acc'
-  rcases checkClause_ok rfl h_check with (h | h)
-  · stop
-
-    done
-  stop
-  done
-
-def checkClause_invariant (τ : PPA) (index : Nat) (hints : Array (Nat × Array Nat)) : Prop :=
-  ∀ (v : IVar), isSet τ v → isSetFor τ v (hints.size - index)
-
-theorem checkClause_ok' {F : ICnf} {σ : PS} {ratHints : Array (Nat × Array Nat)}
-    {τ τ' β β' : PPA} {ratIndex ratIndex' : Nat} {index : Fin F.size}
-    (h_inv : checkClause_invariant τ ratIndex ratHints) :
-    checkClause F σ ratHints ⟨τ, β, ratIndex⟩ index (F.get index) = ok (τ', β', ratIndex') →
-    (checkClause_invariant τ' ratIndex' ratHints ∧
-     F.toPropFun ⊓ τ ≤ (PropFun.bind σ.toSubst (F.get index).toPropFun)) := by
-  sorry
-  done
-
-theorem fold_checkClause_ok' {F : ICnf} {σ : PS} {ratHints : Array (Nat × Array Nat)}
-    {τ β : PPA} {ratIndex : Nat}
-    (h_inv : checkClause_invariant τ 0 ratHints) :
-    F.foldlIdxM (init := (τ, β, 0)) (checkClause F σ ratHints) = ok (τ', β', ratIndex) →
-      F.toPropFun ⊓ τ ≤ (PropFun.bind σ.toSubst F) := by
-  sorry
-  done
-
-
-theorem SR_core' {F : ICnf} {C : IClause} :
-    (∃ σ : (IVar → PropForm IVar), PropFun.bind σ C = ⊤ ∧ F.toPropFun ⊓ Cᶜ ≤ PropFun.bind σ F) →
+-- TODO: Exists a PS, or forall PS that meet the condition?
+-- TODO: Can be "generalized" to one for (IVar → PropForm IVar), or maybe just substitutions in general
+theorem SR_core {F : ICnf} {C : IClause} {σ : PS} :
+    PropFun.substL C σ.toSubst = ⊤ → F.toPropFun ⊓ Cᶜ ≤ PropFun.substL F σ.toSubst →
     eqsat F (F ⊓ C.toPropFun) := by
-  rintro ⟨σ, hC, hFC⟩
+  intro hC hFC
   constructor
   · rintro ⟨τ, hτF⟩
     by_cases hτC : τ ⊨ C.toPropFun
@@ -503,533 +188,313 @@ theorem SR_core' {F : ICnf} {C : IClause} :
       rw [satisfies_conj]
       exact ⟨hτF, hτC⟩
     · replace hFC := entails_ext.mp hFC τ
-      simp [satisfies_conj, and_imp, -satisfies_bind] at hFC
+      simp [satisfies_conj, and_imp, -satisfies_substL] at hFC
       replace hFC := hFC hτF hτC
-      have : τ ⊨ PropFun.bind σ C := by rw [hC]; rfl
+      have : τ ⊨ PropFun.substL C σ.toSubst := by rw [hC]; rfl
       simp at hFC this
-      use PropAssignment.preimage (fun x => ⟦σ x⟧) τ
+      use PropAssignment.subst (fun x => ⟦σ.toSubst x⟧) τ
       rw [satisfies_conj]
       exact ⟨hFC, this⟩
   · rintro ⟨τ, hτ⟩
     rw [satisfies_conj] at hτ
     exact ⟨τ, hτ.1⟩
 
--- IClause × Array ILit × Array (IVar × ILit) × Array Nat × Array (Nat × Array Nat)
--- For the line to continue checking, the clause to be added must be redundant
-theorem checkLine_ok {F : ICnf} {τ β : PPA} {σ : PS} {line : SRLine} {S : SRState}
-    (hF : F ≠ #[]) : -- TODO remove hyp later? But we have to start with UNSAT formula
-    checkLine ⟨F, τ, β, σ⟩ line = ok S → eqsat F.toPropFun (F.toPropFun ⊓ line.1) := by
-  let ⟨C, w_tf, w_maps, up, rats⟩ := line
-  simp [checkLine]
-  split <;> try simp
-  · by_cases hC : C = #[] <;> simp [hC]
-    rename PPA => τ'
-    rename Array.foldlM _ _ _ = _ => h_fold
-    rintro rfl
-    have := fold_UP_checked h_fold
-    simp [assumeNegatedClause_spec τ.reset C rats.size] at this
-    exact eqsat_of_entails (le_iff_inf_compl_eq_bot.mpr this)
-  · rename PPA => τC
-    rename _ => hτC_UP
-    have hτC := fold_UP_ok hτC_UP
-    simp [assumeNegatedClause_spec τ.reset C rats.size] at hτC
-    by_cases hC : C = #[] <;> simp [hC]
-    -- TODO: I want to use split here, but it renames the PPA's in the ok, and I can't rename τ' as a result
-    --split <;> try simp
-    match heq : F.foldlIdxM (checkClause F (assumeWitness σ w_tf w_maps) rats) (τC, β, 0) 0 F.size with
-    | done _ => simp
-    | ok (τ', β', index) =>
-    simp
-    split <;> try simp
-    rename _ = w_tf[0]? => h_pivot
-    rintro rfl
-    apply SR_core'
-    use (assumeWitness σ w_tf w_maps).toSubst
-    constructor
-    · sorry -- Need assumeWitness_spec for this, but because we check the pivot, this is an easy lemma
-      done
-    have h_inv : checkClause_invariant τC 0 rats := by
-      --simp [checkClause_invariant]
-      sorry
-      done
-    have : F.toPropFun ⊓ (F.toPropFun ⊓ C.toPropFunᶜ) ≤ F.toPropFun ⊓ τC := inf_le_inf_left (Cnf.toPropFun F) hτC
-    rw [← inf_assoc, inf_idem] at this
-    exact le_trans this (fold_checkClause_ok' h_inv heq)
-    done
-
-/--
-    split <;> try simp
-    rename _ = w_tf[0]? => h_pivot
-    rintro rfl
-    apply SR_core'
-    use (assumeWitness σ w_tf w_maps).toSubst
-    constructor
-    · sorry -- Need assumeWitness_spec for this, but because we check the pivot, this is an easy lemma
-      done
-    --rename _ = ok _ => heq  -- Use when splitting
-    have ⟨F⟩ := F
-    rw [Array.foldlIdxM, Array.foldlM_eq_foldlM_data] at heq
-    induction' F with C' CS ih generalizing τ β σ
-    · simp at hF
-    · match CS with
-      | [] =>
-        simp at heq
-
-        have hC'_eq : C' = #[C'].get ⟨0, by simp⟩ := rfl
-        --conv at heq => lhs; rhs; rw [hC'_eq]
-        have := (checkClause_ok' h_inv heq).2
-        simp at this hτC ⊢
-        apply le_trans _ this
-        have : C'.toPropFun = C'.toPropFun ⊓ C'.toPropFun := inf_idem.symm
-        conv => lhs; lhs; rw [this]
-        rw [inf_assoc]
-        exact inf_le_inf_left (Clause.toPropFun C') hτC
-        done
-      | C'' :: CS =>
-        clear hF
-        simp at heq
-        have : { data := C'' :: CS } ≠ #[] := by sorry
-        have := ih this
-
-        done
-
-      done
-    done
+theorem assumeWitness_subst {C : IClause} (hC : 0 < C.size) :
+      ∀ σ A₁ A₂, PropFun.substL C.toPropFun (assumeWitness σ (C.get ⟨0, hC⟩) A₁ A₂).toSubst = ⊤ := by
+  intro σ A₁ A₂
+  rw [assumeWitness]
+  simp [PropFun.ext_iff]
+  intro τ
+  rw [Clause.satisfies_iff]
+  use C.get ⟨0, hC⟩
+  constructor
+  · simp [← Array.mem_data]; exact Array.getElem_mem_data C hC
+  · simp [LitVar.satisfies_iff, PropAssignment.subst]
+    sorry
   done
-  stop
-  split at h_fold <;> try contradiction
-  · rename _ => h
-    rename Array.foldlM _ _ _ = _ => h_fold
-    split at h <;> try contradiction
-    · injection h with h
-      injection h with hF hτ hβ hσ
-      subst hF
-      simp [le_iff_inf_compl_le_bot]
-      have := fold_UP_checked h_fold
-      rwa [assumeNegatedClause_spec, le_bot_iff] at this
-  · rename _ => h
-    rename PPA => τ₁
-    rename Array.foldlM _ _ _ = _ => h_fold
-    have := fold_UP_ok h_fold
-    rw [assumeNegatedClause_spec] at this
-    split at h <;> try contradiction
-    stop
-  stop
-  done -/
 
--- For the line to finish checking, the empty clause must be derived
-theorem checkLine_done_true {F : ICnf} {τ β : PPA} {σ : PS} {line : SRLine} :
-    checkLine (SRState.mk F τ β σ) line = done true → F.toPropFun = ⊥ := by
-  let ⟨C, w_tf, w_maps, up, rats⟩ := line
-  simp [checkLine]
-  split <;> try simp
-  · by_cases hC : C = #[] <;> simp [hC]
-    rename PPA => τ'
-    rename _ = done (τ', checked) => heq
-    have := fold_UP_checked heq
-    simp [hC] at this
-    sorry
-    --exact this
-  · by_cases hC : C = #[] <;> simp [hC]
-    split
-    --<;> simp
-    sorry
-    done
+-- TODO: Is the standard `≤ ⊥` or `= ⊥`?
+theorem applyUPHint_checked {F : ICnf} {offset : Nat} {τ τ' : PPA} {hint : Nat} :
+    applyUPHint F offset τ hint = .error (τ', .checked) →
+      τ = τ' ∧ F.toPropFun ⊓ τ ≤ ⊥ := by
+  rw [applyUPHint]
+  split <;> simp
+  split <;> simp
+  rintro rfl; use rfl
+  rename hint < F.size => h_hint
+  rename (unitProp τ _ = _) => h_up
+  have := contradiction_of_UP_falsified h_up
+  rw [inf_comm] at this
+  rw [← le_bot_iff]
+  exact le_trans (inf_le_inf_right τ.toPropFun (Cnf.ith_le ⟨hint, h_hint⟩)) this
 
--- For the proof to check, the clause must be UNSAT
-theorem checkProof_done_true {F : ICnf} {τ β : PPA} {σ : PS} {proof : Array SRLine} :
-    proof.foldlM (init := SRState.mk F τ β σ) checkLine = done true → F.toPropFun = ⊥ := by
-  have ⟨proof⟩ := proof
+-- TODO: Do we need everything in our spec?
+-- Also, the spec is not strong enough to derive ge_of_applyUPHint_ok because
+-- it doesn't comment on the state of F[hint]. See
+theorem applyUPHint_ok {F : ICnf} {offset : Nat} {τ τ' : PPA} {hint : Nat} :
+    applyUPHint F offset τ hint = .ok τ' →
+      --∃ l, l ∈ F[hint] ∧ τ.litValue? l = none ∧ τ' = τ.setLitFor l offset
+      ∃ l, τ.litValue? l = none ∧ τ' = τ.setLitFor l offset := by
+  rw [applyUPHint]
+  split <;> simp
+  split <;> simp
+  rename hint < F.size => h_hint
+  rename ILit => lit
+  rename (unitProp τ _ = _) => h_up
+  rintro rfl
+  rcases extended_of_UP_unit h_up with ⟨_, h₂, _⟩
+  exact ⟨lit, h₂, rfl⟩
+
+theorem ge_of_applyUPHint_ok {F : ICnf} {offset : Nat} {τ τ' : PPA} {hint : Nat} :
+    applyUPHint F offset τ hint = .ok τ' → F.toPropFun ⊓ τ ≤ τ' := by
+  rw [applyUPHint]
+  split <;> simp
+  split <;> simp
+  rename hint < F.size => h_hint
+  rename ILit => lit
+  rename (unitProp τ _ = _) => h_up
+  rintro rfl
+  rcases extended_of_UP_unit h_up with ⟨_, h₂, h₃⟩
+  rw [toPropFun_setLitFor_eq_setLit, toPropFun_setLit_of_none h₂]
+  conv at h₃ => rhs; rw [inf_comm]
+  apply le_trans _ h₃
+  apply inf_le_inf_right
+  exact Cnf.ith_le ⟨hint, h_hint⟩
+
+-- TODO: Package up τ = τ' invariants into "agreeOn" or "unchanged" or something
+theorem fold_UP_checked {F : ICnf} {A : Array Nat} {offset : Nat} {τ τ' : PPA} :
+    A.foldlM (init := τ) (applyUPHint F offset) = error (τ', .checked) →
+      F.toPropFun ⊓ τ ≤ ⊥ ∧ extended τ τ' offset := by
+  have ⟨A⟩ := A
   rw [Array.foldlM_eq_foldlM_data]
-  induction' proof with line lines ih generalizing F τ β σ
-  <;> simp
-  match h_line : checkLine (SRState.mk F τ β σ) line with
-  | done false => intro h; injection h; contradiction
-  | done true => exact (fun _ => checkLine_done_true h_line)
-  | ok S' => exact (fun h => le_bot_iff.mp (ih h ▸ checkLine_ok h_line))
+  induction' A with hint hints ih generalizing τ
+  · simp [pure, Except.pure]
+  · simp [-le_bot_iff]
+    intro h
+    match h_apply : applyUPHint F offset τ hint with
+    | error (τ₁, .checked) =>
+      rcases applyUPHint_checked h_apply with ⟨rfl, hτ⟩
+      use hτ
+      simp [h_apply] at h; injection h; rename _ => h
+      injection h; rename τ = τ' => heq; subst heq
+      simp [PPA.extended]
+      intro v hcon h
+      exact absurd h hcon
+    | error (τ₁, .checkError) =>
+      simp [h_apply] at h; injection h; rename _ => h
+      injection h
+      contradiction
+    | ok τ₁ =>
+      rcases applyUPHint_ok h_apply with ⟨l, hl, rfl⟩
+      -- TODO: What is a better hyp/spec?
+      have hFτ := ge_of_applyUPHint_ok h_apply
+      simp [h_apply] at h
+      rcases ih h with ⟨ih₁, ih₂⟩
+      rw [toPropFun_setLitFor_eq_setLit, toPropFun_setLit_of_none hl, ← inf_assoc] at ih₁
+      rw [toPropFun_setLitFor_eq_setLit, toPropFun_setLit_of_none hl] at hFτ
+      have := inf_le_inf_left F.toPropFun hFτ
+      simp_rw [← inf_assoc, inf_idem] at this
+      exact ⟨le_trans this ih₁, extended_trans (extended_setLitFor_of_none hl offset) ih₂⟩
 
-theorem checkProof_correct (F : ICnf) (proof : Array SRLine) :
-    checkProof F proof = true → F.toPropFun = ⊥ := by
-  simp only [checkProof]
+theorem fold_UP_ok {F : ICnf} {A : Array Nat} {offset : Nat} {τ τ' : PPA} :
+    A.foldlM (init := τ) (applyUPHint F offset) = ok τ' →
+      F.toPropFun ⊓ τ ≤ τ' ∧ extended τ τ' offset := by
+  have ⟨A⟩ := A
+  rw [Array.foldlM_eq_foldlM_data]
+  induction' A with hint hints ih generalizing τ
+  · simp [pure, Except.pure]; rintro rfl; exact ⟨inf_le_right, extended_refl _ _⟩
+  · simp
+    intro h
+    match h_apply : applyUPHint F offset τ hint with
+    | error _ => simp [h_apply] at h; injection h
+    | ok τ₁ =>
+      simp [h_apply] at h
+      rcases ih h with ⟨ih₁, ih₂⟩
+      rcases applyUPHint_ok h_apply with ⟨l, hl, rfl⟩
+      have := inf_le_inf_left F.toPropFun (ge_of_applyUPHint_ok h_apply)
+      rw [← inf_assoc, inf_idem] at this
+      exact ⟨le_trans this ih₁, extended_trans (extended_setLitFor_of_none hl offset) ih₂⟩
+
+theorem assumeRATClause_ok {C : IClause} {σ : PS} {τ τ' : PPA} :
+    assumeRATClause C σ τ = ok τ' →
+      τ.toPropFun ⊓ (PropFun.substL C σ.toSubst)ᶜ ≤ τ' ∧ extended τ τ' 0 := by
+  have ⟨C⟩ := C
+  rw [assumeRATClause, Array.foldlM_eq_foldlM_data]
+  induction' C with l ls ih generalizing τ
+  · simp [pure, Except.pure]; rintro rfl; exact ⟨le_refl _, extended_refl _ _⟩
+  · simp; split <;> rename _ => hσ
+    · intro hcon; injection hcon
+    · intro h
+      rw [litValue_fls_iff] at hσ
+      simp [hσ]
+      exact ih h
+    · rename ILit => mapped_lit
+      rw [litValue_lit_iff] at hσ
+      simp [hσ]
+      split <;> rename _ => h_mapped_lit <;> try simp
+      · intro hcon; injection hcon
+      · intro h
+        rcases ih h with ⟨ih₁, ih₂⟩
+        constructor
+        · apply le_trans _ ih₁
+          apply inf_le_inf_left
+          exact inf_le_right
+        · exact ih₂
+      · intro h
+        rcases ih h with ⟨ih₁, ih₂⟩
+        rw [← litValue?_negate_none_iff] at h_mapped_lit
+        simp [toPropFun_setLit_of_none h_mapped_lit, inf_assoc] at ih₁
+        exact ⟨ih₁, extended_trans (extended_setLitFor_of_none h_mapped_lit 0) ih₂⟩
+
+theorem assumeRATClause_error {C : IClause} {σ : PS} {τ τ' : PPA} :
+    assumeRATClause C σ τ = error τ' →
+      τ.toPropFun ≤ (PropFun.substL C σ.toSubst) ∧ extended τ τ' 0 := by
+  have ⟨C⟩ := C
+  rw [assumeRATClause, Array.foldlM_eq_foldlM_data]
+  induction' C with l ls ih generalizing τ
+  · simp [pure, Except.pure]
+  · simp; split <;> rename _ => hσ
+    · intro h; injection h; rename _ => h; subst h
+      rw [litValue_tr_iff] at hσ
+      simp [hσ]
+    · intro h
+      rw [litValue_fls_iff] at hσ
+      simp [hσ]
+      exact ih h
+    · rename ILit => mapped_lit
+      rw [litValue_lit_iff] at hσ
+      simp [hσ]
+      split <;> rename _ => h_mapped_lit <;> try simp
+      · intro h; injection h; rename _ => h; subst h
+        rw [litValue?_true_iff] at h_mapped_lit
+        exact ⟨le_trans h_mapped_lit le_sup_left, extended_refl _ _⟩
+      · intro h
+        rw [litValue?_false_iff] at h_mapped_lit
+        rcases ih h with ⟨ih₁, ih₂⟩
+        exact ⟨le_trans ih₁ le_sup_right, ih₂⟩
+      · intro h
+        rw [← litValue?_negate_none_iff] at h_mapped_lit
+        rcases ih h with ⟨ih₁, ih₂⟩
+        simp [toPropFun_setLit_of_none h_mapped_lit] at ih₁
+        constructor
+        · exact sdiff_le_iff.mp ih₁
+        · exact extended_trans (extended_setLitFor_of_none h_mapped_lit 0) ih₂
+
+-- Check each clause in the formula.
+-- C is the current clause in the formula to be checked for the RAT property under σ and τ
+-- If C is reduced by σ, then it is RAT. Find a RAT hint and uses the RAT UP hints to derive contradiction.
+--def checkClause (F : ICnf) (σ : PS) (ratHints : Array (Nat × Array Nat))
+--    (p : PPA × Nat) (index : Fin F.size) (C : IClause) : Except Unit (PPA × Nat)
+
+theorem checkClause_ok {F : ICnf} {σ : PS} {ratHints : Array (Nat × Array Nat)}
+    {τ τ' : PPA} {ratIndex ratIndex' index index' bc bc' : Nat} {C : IClause} :
+    C ∈ F → uniform τ ((ratHints.size + 1) - bc) →
+      checkClause F σ ratHints ⟨τ, ratIndex, index, bc⟩ C = ok (τ', ratIndex', index', bc') →
+      F.toPropFun ⊓ τ ≤ PropFun.substL C σ.toSubst ∧
+      ((bc' = bc ∧ τ' = τ) ∨
+       (bc' = bc + 1 ∧ uniform τ' ((ratHints.size + 1) - bc') ∧ τ'.toPropFun = τ.toPropFun)) := by
+  intro hC h_uni
+  simp [checkClause]
+  split <;> rename _ => h_red
+  · simp; rintro rfl rfl rfl rfl
+    rw [reduce_satisfied_iff] at h_red
+    rw [h_red]
+    exact ⟨le_top, Or.inl ⟨rfl, rfl⟩⟩
+  · simp; rintro rfl rfl rfl rfl
+    rw [reduce_notReduced_iff] at h_red
+    rw [h_red]
+    exact ⟨inf_le_of_left_le (Cnf.le_of_mem hC), Or.inl ⟨rfl, rfl⟩⟩
+  · split <;> rename _ => hbc <;> try simp
+    split <;> rename _ => h_hint <;> try simp
+    rename Fin _ => hint_index
+    have h_bc_lt : 1 < (ratHints.size + 1) - bc := by
+      apply Nat.lt_sub_of_add_lt
+      rw [add_comm]
+      exact Nat.add_lt_add_right hbc 1
+    split <;> rename PPA => τ₂ <;> rename _ => h_RAT_assumption <;> try simp
+    · rintro rfl rfl rfl rfl
+      use inf_le_of_right_le (assumeRATClause_error h_RAT_assumption).1
+      right; use rfl
+      rcases assumeRATClause_error h_RAT_assumption with ⟨_, h₂⟩
+      exact uniform_bump_of_uniform_of_extended h_bc_lt h_uni h₂
+    · split <;> rename PPA => τ₃ <;> rename _ => h_ratHints <;> try simp
+      rintro rfl rfl rfl rfl
+      rcases assumeRATClause_ok h_RAT_assumption with ⟨h_RAT₁, h_RAT₂⟩
+      rcases fold_UP_checked h_ratHints with ⟨h₁, h₂⟩
+      have h_ext := extended_trans h_RAT₂ h₂
+      constructor
+      -- TODO: Standard form can probably remove the need for these operations
+      · rw [inf_compl_le_iff_le_sup, sup_comm, ← inf_compl_le_iff_le_sup, inf_comm] at h_RAT₁
+        rw [← le_compl_iff_inf_le_bot] at h₁
+        exact le_trans (inf_le_inf_right (PPA.toPropFun τ) h₁) h_RAT₁
+      · exact Or.inr ⟨rfl, uniform_bump_of_uniform_of_extended h_bc_lt h_uni h_ext⟩
+
+theorem fold_checkClause_ok {F F' : ICnf} {σ : PS} {ratHints : Array (Nat × Array Nat)}
+    {τ τ' : PPA} {ratIndex ratIndex' index index' bc bc' : Nat} :
+    -- TODO: Additional assumptions on τ, related to C or isSetFor
+    (∀ C ∈ F, C ∈ F') →
+    uniform τ ((ratHints.size + 1) - bc) →
+    F.foldlM (checkClause F' σ ratHints) (τ, ratIndex, index, bc) = ok (τ', ratIndex', index', bc') →
+      F'.toPropFun ⊓ τ ≤ (PropFun.substL F σ.toSubst) := by
+  intro hF h_ext
+  have ⟨F⟩ := F
+  rw [Array.foldlM_eq_foldlM_data]
+  induction' F with C CS ih generalizing τ ratIndex index bc <;> simp
+  match h_check : checkClause F' σ ratHints (τ, ratIndex, index, bc) C with
+  | error _ => intro hcon; injection hcon
+  | ok (τ₂, rI₂, i₂, bc₂) =>
+    simp [← Array.mem_data] at hF
+    rcases hF with ⟨hF₁, hF₂⟩
+    rw [Array.mem_data] at hF₁
+    simp [Array.mem_data] at hF₂
+    have : ∀ C ∈ ({ data := CS } : ICnf), C ∈ F' := by
+      simp [← Array.mem_data]; simp_rw [Array.mem_data]; exact hF₂
+    rcases checkClause_ok hF₁ h_ext h_check with ⟨h₁, h₂⟩
+    rcases h₂ with (⟨rfl, rfl⟩ | ⟨rfl, hτ₂_ext, hτ₂_propfun⟩)
+    · exact fun h => ⟨h₁, ih h_ext this h⟩
+    · intro h
+      use h₁
+      rw [← hτ₂_propfun]
+      exact ih hτ₂_ext this h
+
+-- For the line to continue checking, the clause to be added must be redundant
+theorem checkLine_ok {F : ICnf} {τ : PPA} {σ : PS} {line : SRLine} {S : SRState} :
+    checkLine ⟨F, τ, σ⟩ line = ok S → eqsat F.toPropFun (F.toPropFun ⊓ line.1) := by
+  simp [checkLine]
+  rcases line with ⟨C, w_tf, w_maps, UPhints, RAThints⟩
   split <;> try simp
-  rename _ => h
-  exact checkProof_done_true h
-
-#exit
-
-def SRLine := IClause × List (IVar × ILit) × List IClause × List (IClause × List IClause)
-
--- Set up the partial assignment from the candidate clause
-def step2 (τ : PPA) (C : IClause) (offset : Nat) : PPA := (τ.reset).setNegatedClauseFor C offset
-
--- Perform unit propagation
-def step3UP (offset : Nat) (τ : PPA) (C : IClause) : ResultT Bool PPA :=
-  match τ.unitProp' C offset with
-  | .falsified => done true
-  | .satisfied => done false
-  | .unit _ τ' => ok τ'
-  | .multipleUnassignedLiterals => done false
-
-def step3 (τ : PPA) (L : List IClause) (offset : Nat) : ResultT Bool PPA :=
-  L.foldlM (step3UP offset) τ
-
-def step4 (σ : PS) (w : List (IVar × ILit)) : PS := (σ.reset).setVars w
-
-def step5setup (σ : PS) (τ β : PPA) (C : IClause) : ResultT (PPA × PPA) (PPA × PPA × Bool) :=
-  C.foldlM (init := ⟨τ, β, false⟩) (fun ⟨τ', β', b⟩ lit =>
-    match σ.litValue lit with
-    | .tr => done (τ', β')
-    | .fls => ok (τ', β', true)
-    | .lit l =>
-      match β'.litValue? l with
-      | some true => ok (τ', β', b)
-      | some false => done (τ', β')
-      | none =>
-        match τ'.litValue? l with
-        | some true => done (τ', β')
-        | some false => ok ⟨τ', β'.setLit l, b || (lit = l)⟩
-        | none => ok (τ'.setLit l, β'.setLit l, b || (lit = l)))
-
--- σ is the substitution from step 4
--- τ is the partial assignment initialized in step 2
--- β is the tautology PPA that is kept around each step 5, but reset each time
--- C is the candidate RAT clause
--- L is the list of hinted clauses that should lead to contradiction
-def step5 (σ : PS) (τ β : PPA) (C : IClause) (L : List IClause) : ResultT (PS × PPA × PPA × Bool) PPA :=
-  match step5setup σ τ.bump β.reset C with
-  | done (τ', β') => done (σ, τ', β', true)
-  | ok (τ', β', false) => done (σ, τ', β', true)
-  | ok (τ', β', true) =>
-    L.foldlM (init := τ') (fun τ' Cl =>
-      match τ'.unitProp Cl with
-      | .falsified => done (σ, τ', β', true)
-      | .satisfied => done (σ, τ', β', false)
-      | .multipleUnassignedLiterals => done (σ, τ', β', false)
-      | .unit _ τ'' => ok τ'')
-
-structure SRState where
-  τ : PPA       -- α, or the partial assignment that is set to C each line and extended
-  β : PPA       -- A helper data structure to check for tautology in (C∣σ)
-  σ : PS        -- The substitution witness
-
-inductive SRError
-| malformedLine : String → SRError
-| malformedAtom : String → SRError
-| outOfBoundsId : Nat → SRError
-| outOfBoundsLit : Nat → SRError
-| idNotMonotonic : Nat → SRError
-| doubleDeletion : Nat → SRError
-| err : String → SRError
-
--- TODO: "Macro"-like functions for spot-modifying state?
--- TODO: Update CNF parsing logic to be more "monadic"
-abbrev SRStateT := StateT SRState
-abbrev SRCheckerM := SRStateT <| ResultT Bool
-
-
--- LineM (α) := SRState → ResultT (Bool × SRState) (α × SRState)
-abbrev LineM := SRStateT <| ResultT (Bool × SRState)
-abbrev ProofM := SRStateT <| ResultT Bool
-
---abbrev ereturn {β : Type u} (x : Bool) : ResultT (Bool × SRState) β := do done (x, ← get)
-
--- When we process the unit propagation hints, we can succeed on the line, or fail
--- If we get (done false), then we exit the proof checking at top level
--- If we get (done true), then the clause checks out, and we can skip the line
--- If we get (ok _), then we continue to RAT hints
-def UPHintsToProof (m : LineM Unit) : ProofM Unit := do
-  fun s =>
-  match m s with
-  | ok ⟨_, σ⟩ => ok ⟨(), σ⟩
-  | done ⟨true, σ⟩ => ok ⟨(), σ⟩
-  | done ⟨false, _⟩ => done false
-
--- When checking the RAT hints, we want to end each block having derived contradiction.
--- If we derive contradiction, then we should get back (done true).
--- If we get (done false), some RAT hint failed, so we forward that result.
--- If we get (done true), we derived contradiction. We switch to (ok _) to keep folding.
--- If we get (ok _), then we didn't derive contradiction, so we fail.
-def RATBlock {α : Type _} (m : LineM α) : ProofM Unit := do
-  fun s =>
-  match m s with
-  | ok _ => done false
-  | done ⟨true, σ⟩ => ok ⟨(), σ⟩
-  | done ⟨false, _⟩ => done false
-
--- At the very end of checking every line, we convert a LineM monad into a ProofM monad.
--- If we get (done false), then the proof didn't check at some point, and we forward that result.
--- If we get (done true), then we successfully validated the proof line containing the empty clause.
-      -- Forward along the updated state to keep folding.
--- If we get (ok _), then every line checked, but we didn't find the empty clause. So we fail.
-def LineToProof {α : Type _} (m : LineM α) : ProofM Unit := do
-  fun s =>
-  match m s with
-  | ok ⟨_, _⟩ => done false
-  | done ⟨true, σ⟩ => ok ⟨(), σ⟩
-  | done ⟨false, _⟩ => done false
-
--- Build τ from candidate redundant clause C. Resets from previous line.
-def assumeNegatedClause (C : IClause) (offset : Nat) : SRStateT Id Unit :=
-  modify (fun st => { st with τ := st.τ.reset.setNegatedClauseFor C offset })
-
--- Perform unit propagation with τ on given clause. Expects contradiction or unit
-def applyUPHint (offset : Nat) (C : IClause) : LineM Unit := do
-  match (← get).τ.unitProp' C offset with
-  | .falsified => done (true, ← get)      -- Cayden TODO: How to have function/macro so don't call (← get)?
-  | .satisfied => done (false, ← get)
-  | .unit _ τ' => modify (fun st => { st with τ := τ' })
-  | .multipleUnassignedLiterals => done (false, ← get)
-
-
--- Cayden TODO: Figure out how can be made without | done b => done b
--- Try to derive contradiction through unit propagation hints.
--- Early exit with (done true) will get handled at top-level when checking the line
--- Early exit with (done false) causes the whole proof to stop
-def applyUPHints (L : List IClause) (offset : Nat) : LineM Unit := do
-  match L.foldlM (step3UP offset) (init := (← get).τ) with
-  | ok τ' => modify (fun st => { st with τ := τ' })
-  | done b => done (b, ← get)
-
-
--- An alternate definition that modifies each time rather than folding τ along
--- It does have a Unit as the accumulator...
--- Check which version is faster later
-def applyUPHints' (L : List IClause) (offset : Nat) : LineM Unit :=
-  L.foldlM (fun _ => applyUPHint offset) (init := ())
-
--- Set the witness substitution σ from the provided mapping, resetting σ first
-def assumeWitness (w : List (IVar × ILit)) : SRStateT Id Unit :=
-  modify (fun st => { st with σ := st.σ.setVars w })
-
--- Reduce C under σ, and then check for tautologies (via β) and evaluate under τ
--- If a literal is unassigned by τ, add it to τ for the RAT steps
--- If a literal evaluates to ⊤ under either σ or τ, the clause can be skipped
-def reduceRATClause (C : IClause) : LineM Bool := do
-  modify (fun st => { st with
-    τ := st.τ.bump
-    β := st.β.reset })
-  C.foldlM (init := false) (fun b lit => do
-    match (← get).σ.litValue lit with
-    | .tr => done (true, ← get)
-    | .fls => return true             -- Cayden TODO/Q: Why 'return' here?
-    | .lit l =>
-      match (← get).β.litValue? l with
-      | some true => return b
-      | some false => done (true, ← get)
-      | none =>
-        match (← get).τ.litValue? l with
-        | some true => done (true, ← get)
-        | some false =>
-          modify (fun st => { st with β := st.β.setLit l })
-          return (b || (lit = l))
-        | none =>
-          modify (fun st => { st with
-            τ := st.τ.setLit l
-            β := st.β.setLit l })
-          return (b || (lit = l)))
-
--- σ is the substitution witness
--- τ is the partial assignment (negation of C)
--- β is the tautology PPA that is kept around each step 5, but reset each time
--- C is the candidate RAT clause
--- L is the list of hinted clauses that should lead to contradiction
--- Checks a pair of a RAT clause and a list of clause hints
-def applyRATHint (C : IClause) (L : List IClause) : LineM Unit := do
-  match ← reduceRATClause C with
-  -- The witness σ doesn't reduce C, so we can skip the clause
-  | false => done (true, ← get)
-  -- The witness σ does reduce C
-  | true =>
-    -- Evaluate RAT hints with C loaded into the state
-    L.foldlM (init := ()) (fun _ Cl => do
-      match (← get).τ.unitProp Cl with
-      -- Derived unit prop contradiction
-      | .falsified => done (true, ← get)
-      -- During unit prop, we should never find a hinted clause that is satisfied or not unit/contra
-      | .satisfied => done (false, ← get)
-      | .multipleUnassignedLiterals => done (false, ← get)
-      -- If we find unit, extend the partial assignment
-      | .unit _ τ' => modify (fun st => { st with τ := τ' }))
-
-def McheckLine (l : SRLine) : ProofM Unit := do
-  match l with
-  | ⟨C, w, L, R⟩ =>
-    let offset := R.length
-    let _ := assumeNegatedClause C offset
-    -- If we derive contradiction through UP hints and we exit early through monad,
-    -- then we are done with the line
-    let _ ← UPHintsToProof (applyUPHints' L offset)--
-    -- Now we set up the witness
-    let _ := assumeWitness w
-    -- Now check all RAT hints, holding into the ProofM monad via ExpectDoneTrue
-    let _ ← R.foldlM (init := ()) (fun _ ⟨Cl, H⟩ => RATBlock (applyRATHint Cl H))
-    if C = #[] then done true else return
-
-def McheckLines (lines : List SRLine) : Bool := --SRCheckerM Unit :=
-  let state : SRState := {
-    τ := PPA.new 100
-    β := PPA.new 100
-    σ := PS.new 100
-  }
-
-  match ((lines.foldlM (init := ()) (fun _ line => McheckLine line)) : ProofM Unit) |>.run state with
-  -- If we end up with "okay", then we never validated the empty clause, so the proof didn't check
-  | ok _ => false
-  -- If we exited early with "true", then we validated the empty clause, so the proof checked out
-  | done true => true
-  -- If we exited early with "false", then there was a problem somewhere in the proof, so it didn't check
-  | done false => false
-
-theorem Mchecklines_correct (lines : List SRLine) :
-  McheckLines lines = true →
-
-/-
-
-Overall: returns Bool
-
-for each line:      (has type σ → ResultT Bool Unit, can drop state.
-                     But since ignore "ok" case, could have SRCheckerM Unit := σ → ResultT Bool (Unit × σ))
-  check line        (has type SRCheckerM Unit := σ → ResultT Bool (Unit × σ))
-    step 2: set τ   (has type SRStateT Id Unit := σ → (Unit × σ))  (because can't fail)
-    step 3: unit prop hints
-                    (has type SRCheckerM Unit := σ → ResultT (Bool × σ) (Unit × σ))
-                    (Can fail early (done false), but can't succeed early (except for the line))
-
--/
-
-#exit
-
-/-! # Unit propagation across many clauses -/
-
-/-
-open ResultT MUPResult MUPDone
-
-abbrev UPBox := ResultT MUPDone (Option ILit)
-
-
-def pevalUP (τ : PPA) (unit? : Option ILit) (l : ILit) : UPBox :=
-  match τ.litValue? l with
-  | some true => done .satisfied
-  | some false => ok unit?
-  | none =>
-    match unit? with
-    | none => ok l
-    | some u =>
-      if u = l then ok unit?
-      -- Assume tautology cannot occur in clause, so two unassiged literals exits early
-      else done .multipleUnassignedLiterals
-
-def foldUP (τ : PPA) (C : IClause) := C.foldlM (pevalUP τ) none
-
--/
-
--- Cayden TODO: better name needed
--- Return true if contradiction reached. Otherwise, false
-abbrev LineBox := ResultT Bool PPA
-
-def toPF (F : PropFun IVar) (C : IClause) : PropFun IVar := F ⊓ C.toPropFun
-
-@[simp] theorem toPF_top (C : IClause) : toPF ⊤ C = C.toPropFun := by
-  rw [toPF, top_inf_eq]
-
-def LtoPF (L : List IClause) : PropFun IVar := L.foldl toPF ⊤
-def AtoPF (A : Array IClause) : PropFun IVar := A.foldl toPF ⊤
-
-@[simp] theorem AtoPF_eq_LtoPF (A : Array IClause) : AtoPF A = LtoPF A.data :=
-  Array.foldl_eq_foldl_data _ _ _
-
-@[simp] theorem LtoPF_nil : LtoPF ([] : List IClause) = ⊤ := rfl
-
--- TODO: Make into a single simp?
-theorem LtoPF_init (τ : PropFun IVar) (L : List IClause) :
-    L.foldl toPF τ = τ ⊓ LtoPF L := by
-  induction' L with C CS ih generalizing τ
-  · simp
-  · simp [ih]
-    conv => rhs; rw [LtoPF]
-    rw [List.foldl_cons, ih]
-    simp [toPF, inf_assoc]
-
-@[simp] theorem LtoPF_cons (C : IClause) (L : List IClause) :
-    LtoPF (C :: L) = C.toPropFun ⊓ LtoPF L := by
-  simp [LtoPF]
-  rw [LtoPF_init, LtoPF]
-
-def applyUPHint (τ : PPA) (C : IClause) : LineBox :=
-  match τ.unitProp C with
-  | .falsified => done true
-  | .satisfied => done false
-  | .unit _ τ' => ok τ'
-  | .multipleUnassignedLiterals => done false
-
-def AfoldUPs (τ : PPA) (A : Array IClause) := A.foldlM applyUPHint τ
-def LfoldUPs (τ : PPA) (L : List IClause) := L.foldlM applyUPHint τ
-
-@[simp] theorem Afold_eq_Lfold (τ : PPA) (A : Array IClause) : AfoldUPs τ A = LfoldUPs τ A.data :=
-  Array.foldlM_eq_foldlM_data _ _ _
-
-@[simp] theorem LfoldUPs_nil (τ : PPA) : LfoldUPs τ ([] : List IClause) = ok τ := rfl
-
-theorem unit_of_LfoldUPs_cons_ok {τ τ' : PPA} {C : IClause} {L : List IClause} :
-    LfoldUPs τ (C :: L) = ok τ' → ∃ (l : ILit) (τ'' : PPA), τ.unitProp C = unit l τ'' := by
-  intro h
-  rw [LfoldUPs, List.foldlM_cons, applyUPHint] at h
-  cases hτ : τ.unitProp C <;> simp [hτ] at h <;> try contradiction
-  exact ⟨_, _, rfl⟩
-
-theorem LfoldUPs_cons_of_falsified {τ : PPA} {C : IClause} {L : List IClause} :
-    τ.unitProp C = .falsified → LfoldUPs τ (C :: L) = done true := by
-  intro h; simp [LfoldUPs, List.foldlM_cons, applyUPHint, h]; rfl
-
-theorem LfoldUPs_cons_of_unit {l : ILit} {τ τ' : PPA} {C : IClause} {L : List IClause} :
-    τ.unitProp C = unit l τ' → LfoldUPs τ (C :: L) = LfoldUPs τ' L := by
-  intro h; simp [LfoldUPs, List.foldlM_cons, applyUPHint, h]; rfl
-
-theorem LfoldUPs_ok {τ τ' : PPA} {L : List IClause} :
-    LfoldUPs τ L = ok τ' → (LtoPF L) ⊓ τ ≤ τ' := by
-  induction' L with C CS ih generalizing τ
-  · simp; rintro rfl; exact Eq.ge rfl
-  · intro h
-    rw [LtoPF_cons, inf_comm, ← inf_assoc, inf_comm]
-    rcases unit_of_LfoldUPs_cons_ok h with ⟨l, σ, hτ⟩
-    rw [LfoldUPs_cons_of_unit hτ] at h
-    apply le_trans _ (ih h)
-    have := (extended_of_UP_unit hτ).1
-    rw [inf_comm] at this
-    exact inf_le_inf_left _ this
-
-theorem LfoldUPs_true {τ : PPA} {L : List IClause} :
-    LfoldUPs τ L = done true → LtoPF L ⊓ τ ≤ ⊥ := by
-  induction' L with C CS ih generalizing τ
-  · simp
-  · intro h
-    rw [LfoldUPs, List.foldlM_cons, applyUPHint] at h
-    split at h <;> try injection h <;> try contradiction
-    · rename unitProp τ C = falsified => heq
-      rw [LtoPF_cons, inf_comm, ← inf_assoc]
-      exact le_trans inf_le_left (contradiction_of_UP_falsified heq)
-    · rename ILit => l
-      rename PPA => τ'
-      rename unitProp τ C = unit _ _ => heq
-      have := (extended_of_UP_unit heq).1
-      rw [inf_comm] at this
-      rw [LtoPF_cons, inf_comm, ← inf_assoc, inf_comm]
-      apply le_trans (inf_le_inf_left (LtoPF CS) this)
-      apply ih
-      rw [← h]
-      rfl
-
-theorem AfoldUPs_ok {τ τ' : PPA} {A : Array IClause} :
-    AfoldUPs τ A = ok τ' → AtoPF A ⊓ τ ≤ τ' := by
-  rw [Afold_eq_Lfold, AtoPF_eq_LtoPF]; exact LfoldUPs_ok
-
-theorem AfoldUPs_true {τ : PPA} {A : Array IClause} :
-    AfoldUPs τ A = done true → AtoPF A ⊓ τ ≤ ⊥ := by
-  rw [Afold_eq_Lfold, AtoPF_eq_LtoPF]; exact LfoldUPs_true
-
-abbrev RATBox := ResultT Bool PPA
-
-def RATLine (τ : PPA) (R : List (List IClause)) : RATBox :=
-
+  rename PPA => τ₁
+  rename _ = ok τ₁ => h_assumeNegatedCandidate
+  rcases assumeNegatedClauseFor_ok h_assumeNegatedCandidate with ⟨hC₁, hC₂⟩
+  replace hC₂ := uniform_of_extended_reset hC₂
+  simp at hC₁ hC₂
+  --replace hC₂ := uniform_of_extended_reset hC₂
+  match h_hints : UPhints.foldlM (applyUPHint F (RAThints.size + 1)) τ₁ with
+  | error (_, .checkError) => simp
+  | error (τ', .checked) =>
+    simp; split <;> simp
+    rcases fold_UP_checked h_hints with ⟨h₁, h₂⟩
+    rw [hC₁] at h₁
+    rw [← le_iff_inf_compl_le_bot] at h₁
+    exact fun _ => eqsat_of_entails h₁
+  | ok τ₂ =>
+    simp; split <;> try simp
+    split <;> try simp
+    rename 0 < _ ∧ 0 < _ => h_sizes
+    rcases h_sizes with ⟨hC_size, hw_size⟩
+    match h_RAT : F.foldlM (checkClause F (assumeWitness σ C[0] w_tf w_maps) RAThints) (τ₂, 0, 0, 0) with
+    | error () => simp
+    | ok (τ₃, idx₃) =>
+      split <;> try simp
+      rename _ => h_ok; simp at h_ok; rcases h_ok with ⟨rfl, rfl⟩
+      rcases fold_UP_ok h_hints with ⟨h₁, h₂⟩
+      rw [hC₁] at h₁
+      intro
+      apply SR_core (assumeWitness_subst hC_size σ w_tf w_maps)
+      replace hC₂ : uniform τ₂ ((RAThints.size + 1) - 0) := uniform_of_uniform_of_extended hC₂ h₂
+      have hFC_le_Fτ₂ : F.toPropFun ⊓ (C.toPropFun)ᶜ ≤ F.toPropFun ⊓ τ₂ := by
+        have := inf_le_inf_left F.toPropFun h₁
+        rwa [← inf_assoc, inf_idem] at this
+      exact le_trans hFC_le_Fτ₂ (fold_checkClause_ok (by simp) hC₂ h_RAT)
 
 end SR
