lakefile.lean
@@ -12,9 +12,9 @@ lean_lib Examples {
   globs := #[.submodules `Examples]
 }
 
--- Note: `mathlib` and `std` are obtained transitively so that the versions all match up
-require leancolls from git "https://github.com/JamesGallicchio/LeanColls.git" @ "main"
-
 lean_lib Experiments {
   globs := #[.submodules `Experiments]
 }
+
+-- Note: `mathlib` and `std` are obtained transitively so that the versions all match up
+require leancolls from git "https://github.com/JamesGallicchio/LeanColls.git" @ "main"
